added the refinement of functions related to copy_atom_to_operand_nat

Cook_Levin/IMP-_To_SAS+/IMP-_To_IMP--/Binary_Operations_IMP.thy
@@ -10,4 +10,3136 @@ begin
 
 unbundle IMP_Minus_Minus_Com.no_com_syntax
 
-end
+
+subsection copy_var_to_operand
+
+subsubsection copy_var_to_operand_aux1
+
+record copy_var_to_operand_aux1_state=
+copy_var_to_operand_aux1_op::nat
+copy_var_to_operand_aux1_diff::nat
+copy_var_to_operand_aux1_ret::nat
+
+abbreviation "copy_var_to_operand_aux1_prefix \<equiv> ''copy_var_to_operand_aux1_op.''"
+abbreviation "copy_var_to_operand_aux1_op_str \<equiv> ''op''"
+abbreviation "copy_var_to_operand_aux1_diff_str \<equiv> ''diff''"
+abbreviation "copy_var_to_operand_aux1_ret_str \<equiv> ''ret''"
+
+definition "copy_var_to_operand_aux1_imp_state_upd s \<equiv> 
+ (let
+   prod_encode_a' = copy_var_to_operand_aux1_op s;
+   prod_encode_b' = copy_var_to_operand_aux1_diff s;
+   prod_encode_ret' = 0;
+   prod_encode_state = \<lparr>prod_encode_a = prod_encode_a',
+                       prod_encode_b = prod_encode_b',
+                       prod_encode_ret = prod_encode_ret'\<rparr>;
+   prod_encode_ret_state = prod_encode_imp prod_encode_state;
+   var_bit_to_var_tail_n' = prod_encode_ret prod_encode_ret_state;
+   var_bit_to_var_tail_ret' = 0;
+   var_bit_to_var_tail_state = \<lparr>var_bit_to_var_tail_n = var_bit_to_var_tail_n',
+                               var_bit_to_var_tail_ret = var_bit_to_var_tail_ret'\<rparr>;
+   var_bit_to_var_tail_ret_state = var_bit_to_var_tail_imp var_bit_to_var_tail_state;
+
+   cons_h' = var_bit_to_var_tail_ret var_bit_to_var_tail_ret_state;
+   cons_t' = 0;
+   cons_ret' = 0;
+   cons_state = \<lparr>cons_h = cons_h', cons_t = cons_t', cons_ret = cons_ret'\<rparr>;
+   cons_ret_state = cons_imp cons_state;
+
+   copy_var_to_operand_aux1_ret' = cons_ret cons_ret_state;
+   ret = \<lparr>copy_var_to_operand_aux1_op = copy_var_to_operand_aux1_op s,
+         copy_var_to_operand_aux1_diff = copy_var_to_operand_aux1_diff s,
+         copy_var_to_operand_aux1_ret = copy_var_to_operand_aux1_ret'\<rparr>
+  in
+   ret)"
+
+function copy_var_to_operand_aux1_imp 
+ :: "copy_var_to_operand_aux1_state \<Rightarrow> copy_var_to_operand_aux1_state" where 
+"copy_var_to_operand_aux1_imp s = 
+  (let
+     ret = copy_var_to_operand_aux1_imp_state_upd s
+   in
+    ret)" by simp+
+termination 
+  by (relation "measure copy_var_to_operand_aux1_op", simp)
+
+declare copy_var_to_operand_aux1_imp.simps[simp del]
+
+lemma copy_var_to_operand_aux1_imp_correct[let_function_correctness]:
+  "copy_var_to_operand_aux1_ret (copy_var_to_operand_aux1_imp s)
+    = ((var_bit_to_var_tail (prod_encode (
+        (copy_var_to_operand_aux1_op s), (copy_var_to_operand_aux1_diff s)))) ## 0)"
+apply (subst copy_var_to_operand_aux1_imp.simps copy_var_to_operand_aux1_imp_state_upd_def)+
+apply (auto simp add: Let_def var_bit_to_var_tail_imp_correct 
+  cons_imp_correct prod_encode_imp_correct)
+done 
+
+definition "copy_var_to_operand_aux1_imp_state_upd_time t s \<equiv> 
+ (let
+   prod_encode_a' = copy_var_to_operand_aux1_op s;
+   t = t + 2;
+   prod_encode_b' = copy_var_to_operand_aux1_diff s;
+   t = t + 2;
+   prod_encode_ret' = 0;
+   t = t + 2;
+   prod_encode_state = \<lparr>prod_encode_a = prod_encode_a',
+                       prod_encode_b = prod_encode_b',
+                       prod_encode_ret = prod_encode_ret'\<rparr>;
+   prod_encode_ret_state = prod_encode_imp prod_encode_state;
+   t = t + prod_encode_imp_time 0 prod_encode_state;
+
+   var_bit_to_var_tail_n' = prod_encode_ret prod_encode_ret_state;
+   t = t + 2;
+   var_bit_to_var_tail_ret' = 0;
+   t = t + 2;
+   var_bit_to_var_tail_state = \<lparr>var_bit_to_var_tail_n = var_bit_to_var_tail_n',
+                               var_bit_to_var_tail_ret = var_bit_to_var_tail_ret'\<rparr>;
+   var_bit_to_var_tail_ret_state = var_bit_to_var_tail_imp var_bit_to_var_tail_state;
+   t = t + var_bit_to_var_tail_imp_time 0 var_bit_to_var_tail_state;
+
+   cons_h' = var_bit_to_var_tail_ret var_bit_to_var_tail_ret_state;
+   t = t + 2;
+   cons_t' = 0;
+   t = t + 2;
+   cons_ret' = 0;
+   t = t + 2;
+   cons_state = \<lparr>cons_h = cons_h', cons_t = cons_t', cons_ret = cons_ret'\<rparr>;
+   cons_ret_state = cons_imp cons_state;
+   t = t + cons_imp_time 0 cons_state;
+
+   copy_var_to_operand_aux1_ret' = cons_ret cons_ret_state;
+   t = t + 2;
+   ret = \<lparr>copy_var_to_operand_aux1_op = copy_var_to_operand_aux1_op s,
+         copy_var_to_operand_aux1_diff = copy_var_to_operand_aux1_diff s,
+         copy_var_to_operand_aux1_ret = copy_var_to_operand_aux1_ret'\<rparr>
+  in
+   t)"
+
+function copy_var_to_operand_aux1_imp_time 
+ :: "nat \<Rightarrow> copy_var_to_operand_aux1_state \<Rightarrow> nat" where 
+"copy_var_to_operand_aux1_imp_time t s = 
+  (let
+     ret = copy_var_to_operand_aux1_imp_state_upd s;
+     t = t + copy_var_to_operand_aux1_imp_state_upd_time 0 s
+   in
+    t)" by auto
+termination 
+  by (relation "measure (copy_var_to_operand_aux1_op \<circ> snd)", simp)
+
+definition "copy_var_to_operand_aux1_IMP_Minus \<equiv> 
+  (prod_encode_prefix @ prod_encode_a_str) ::= A (V copy_var_to_operand_aux1_op_str);;
+  (prod_encode_prefix @ prod_encode_b_str) ::= A (V copy_var_to_operand_aux1_diff_str);;
+  (prod_encode_prefix @ prod_encode_ret_str) ::= A (N 0);;
+  invoke_subprogram prod_encode_prefix prod_encode_IMP_Minus;;
+  
+  (var_bit_to_var_tail_prefix @ var_bit_to_var_tail_n_str) ::= A (V (prod_encode_prefix @ prod_encode_ret_str));;
+  (var_bit_to_var_tail_prefix @ var_bit_to_var_tail_ret_str) ::= A (N 0);;
+  invoke_subprogram var_bit_to_var_tail_prefix var_bit_to_var_tail_IMP_Minus;;
+  
+  (cons_prefix @ cons_h_str) ::= A (V (var_bit_to_var_tail_prefix @ var_bit_to_var_tail_ret_str));;
+  (cons_prefix @ cons_t_str) ::= A (N 0);;
+  (cons_prefix @ cons_ret_str) ::= A (N 0);;
+  invoke_subprogram cons_prefix cons_IMP_Minus;;
+  
+  copy_var_to_operand_aux1_ret_str ::= A (V (cons_prefix @ cons_ret_str))"
+
+abbreviation "copy_var_to_operand_aux1_IMP_vars \<equiv> 
+  {copy_var_to_operand_aux1_op_str, copy_var_to_operand_aux1_diff_str, copy_var_to_operand_aux1_ret_str}"
+
+definition "copy_var_to_operand_aux1_imp_to_HOL_state p s \<equiv> 
+  \<lparr>copy_var_to_operand_aux1_op = s (add_prefix p copy_var_to_operand_aux1_op_str),
+  copy_var_to_operand_aux1_diff = s (add_prefix p copy_var_to_operand_aux1_diff_str),
+  copy_var_to_operand_aux1_ret = s (add_prefix p copy_var_to_operand_aux1_ret_str)\<rparr>"
+
+lemmas copy_var_to_operand_aux1_state_translators =
+  copy_var_to_operand_aux1_imp_to_HOL_state_def
+  cons_imp_to_HOL_state_def
+  var_bit_to_var_tail_imp_to_HOL_state_def 
+  prod_encode_imp_to_HOL_state_def
+
+lemma copy_var_to_operand_aux1_IMP_Minus_correct_function:
+  "(invoke_subprogram p copy_var_to_operand_aux1_IMP_Minus, s) \<Rightarrow>\<^bsup>t\<^esup> s' \<Longrightarrow>
+     s' (add_prefix p copy_var_to_operand_aux1_ret_str)
+      = copy_var_to_operand_aux1_ret (copy_var_to_operand_aux1_imp (copy_var_to_operand_aux1_imp_to_HOL_state p s))"
+  apply (simp only: copy_var_to_operand_aux1_imp.simps copy_var_to_operand_aux1_imp_state_upd_def)
+  apply (simp only: copy_var_to_operand_aux1_IMP_Minus_def prefix_simps)
+  apply (erule Seq_E)+
+  apply (erule prod_encode_IMP_Minus_correct[where vars=copy_var_to_operand_aux1_IMP_vars])
+  subgoal premises p using p(12) by fastforce
+  apply (erule var_bit_to_var_tail_IMP_Minus_correct[where vars=copy_var_to_operand_aux1_IMP_vars])
+  subgoal premises p using p(14) by fastforce
+  apply (erule cons_IMP_Minus_correct[where vars=copy_var_to_operand_aux1_IMP_vars])
+  subgoal premises p using p(16) by fastforce
+  apply (force simp add: copy_var_to_operand_aux1_state_translators Let_def)
+  done 
+
+lemma copy_var_to_operand_aux1_IMP_Minus_correct_time:
+  "(invoke_subprogram p copy_var_to_operand_aux1_IMP_Minus, s) \<Rightarrow>\<^bsup>t\<^esup> s' \<Longrightarrow>
+     t = copy_var_to_operand_aux1_imp_time 0 (copy_var_to_operand_aux1_imp_to_HOL_state p s)"
+  apply (simp only: copy_var_to_operand_aux1_imp_time.simps copy_var_to_operand_aux1_imp_state_upd_time_def)
+  apply (simp only: copy_var_to_operand_aux1_IMP_Minus_def prefix_simps)
+  apply (erule Seq_tE)+
+  apply (erule prod_encode_IMP_Minus_correct[where vars=copy_var_to_operand_aux1_IMP_vars])
+  subgoal premises p using p(23) by fastforce
+  apply (erule var_bit_to_var_tail_IMP_Minus_correct[where vars=copy_var_to_operand_aux1_IMP_vars])
+  subgoal premises p using p(25) by fastforce
+  apply (erule cons_IMP_Minus_correct[where vars=copy_var_to_operand_aux1_IMP_vars])
+  subgoal premises p using p(27) by fastforce
+  apply (force simp add: copy_var_to_operand_aux1_state_translators Let_def)
+  done 
+
+lemma copy_var_to_operand_aux1_IMP_Minus_correct:
+  "\<lbrakk>(invoke_subprogram (p1 @ p2) copy_var_to_operand_aux1_IMP_Minus, s) \<Rightarrow>\<^bsup>t\<^esup> s';
+    \<And>v. v \<in> vars \<Longrightarrow> \<not> (set p2 \<subseteq> set v);
+     \<lbrakk>t = (copy_var_to_operand_aux1_imp_time 0 (copy_var_to_operand_aux1_imp_to_HOL_state (p1 @ p2) s));
+      s' (add_prefix (p1 @ p2) copy_var_to_operand_aux1_ret_str) =
+        copy_var_to_operand_aux1_ret
+          (copy_var_to_operand_aux1_imp (copy_var_to_operand_aux1_imp_to_HOL_state (p1 @ p2) s));
+      \<And>v. v \<in> vars \<Longrightarrow> s (add_prefix p1 v) = s' (add_prefix p1 v)\<rbrakk>
+     \<Longrightarrow> P\<rbrakk> \<Longrightarrow> P"
+  using copy_var_to_operand_aux1_IMP_Minus_correct_function 
+      copy_var_to_operand_aux1_IMP_Minus_correct_time
+       set_mono_prefix
+  by (smt (verit, ccfv_SIG) com_add_prefix_valid_subset com_only_vars)
+
+subsubsection copy_var_to_operand_aux2
+
+record copy_var_to_operand_aux2_state=
+copy_var_to_operand_aux2_op::nat
+copy_var_to_operand_aux2_diff::nat
+copy_var_to_operand_aux2_ret::nat
+
+abbreviation "copy_var_to_operand_aux2_prefix \<equiv> ''copy_var_to_operand_aux2_op.''"
+abbreviation "copy_var_to_operand_aux2_op_str \<equiv> ''op''"
+abbreviation "copy_var_to_operand_aux2_diff_str \<equiv> ''diff''"
+abbreviation "copy_var_to_operand_aux2_ret_str \<equiv> ''ret''"
+
+definition "copy_var_to_operand_aux2_imp_state_upd s \<equiv> 
+ (let
+   prod_encode_a' = copy_var_to_operand_aux2_op s;
+   prod_encode_b' = copy_var_to_operand_aux2_diff s;
+   prod_encode_ret' = 0;
+   prod_encode_state = \<lparr>prod_encode_a = prod_encode_a',
+                       prod_encode_b = prod_encode_b',
+                       prod_encode_ret = prod_encode_ret'\<rparr>;
+   prod_encode_ret_state = prod_encode_imp prod_encode_state;
+   operand_bit_to_var_tail_n' = prod_encode_ret prod_encode_ret_state;
+   operand_bit_to_var_tail_ret' = 0;
+   operand_bit_to_var_tail_state = \<lparr>operand_bit_to_var_tail_n = operand_bit_to_var_tail_n',
+                               operand_bit_to_var_tail_ret = operand_bit_to_var_tail_ret'\<rparr>;
+   operand_bit_to_var_tail_ret_state = operand_bit_to_var_tail_imp operand_bit_to_var_tail_state;
+
+   cons_h' = 1;
+   cons_t' = 0;
+   cons_ret' = 0;
+   cons_state = \<lparr>cons_h = cons_h', cons_t = cons_t', cons_ret = cons_ret'\<rparr>;
+   cons_ret_state = cons_imp cons_state;
+
+   cons_h' = operand_bit_to_var_tail_ret operand_bit_to_var_tail_ret_state;
+   cons_t' = cons_ret cons_ret_state;
+   cons_ret' = 0;
+   cons_state = \<lparr>cons_h = cons_h', cons_t = cons_t', cons_ret = cons_ret'\<rparr>;
+   cons_ret_state = cons_imp cons_state;
+
+   cons_h' = 1;
+   cons_t' = cons_ret cons_ret_state;
+   cons_ret' = 0;
+   cons_state = \<lparr>cons_h = cons_h', cons_t = cons_t', cons_ret = cons_ret'\<rparr>;
+   cons_ret_state = cons_imp cons_state;
+
+   copy_var_to_operand_aux2_ret' = cons_ret cons_ret_state;
+   ret = \<lparr>copy_var_to_operand_aux2_op = copy_var_to_operand_aux2_op s,
+         copy_var_to_operand_aux2_diff = copy_var_to_operand_aux2_diff s,
+         copy_var_to_operand_aux2_ret = copy_var_to_operand_aux2_ret'\<rparr>
+  in
+   ret)"
+
+function copy_var_to_operand_aux2_imp 
+ :: "copy_var_to_operand_aux2_state \<Rightarrow> copy_var_to_operand_aux2_state" where 
+"copy_var_to_operand_aux2_imp s = 
+  (let
+     ret = copy_var_to_operand_aux2_imp_state_upd s
+   in
+    ret)" by simp+
+termination 
+  by (relation "measure copy_var_to_operand_aux2_op", simp)
+
+declare copy_var_to_operand_aux2_imp.simps[simp del]
+
+lemma copy_var_to_operand_aux2_imp_correct[let_function_correctness]:
+  "copy_var_to_operand_aux2_ret (copy_var_to_operand_aux2_imp s)
+    = (1 ## (operand_bit_to_var_tail (prod_encode (
+        (copy_var_to_operand_aux2_op s), (copy_var_to_operand_aux2_diff s)))) ## 1 ## 0)"
+apply (subst copy_var_to_operand_aux2_imp.simps copy_var_to_operand_aux2_imp_state_upd_def)+
+apply (auto simp add: Let_def operand_bit_to_var_tail_imp_correct 
+  cons_imp_correct prod_encode_imp_correct)
+done 
+
+definition "copy_var_to_operand_aux2_imp_state_upd_time t s \<equiv> 
+ (let
+   prod_encode_a' = copy_var_to_operand_aux2_op s;
+   t = t + 2;
+   prod_encode_b' = copy_var_to_operand_aux2_diff s;
+   t = t + 2;
+   prod_encode_ret' = 0;
+   t = t + 2;
+   prod_encode_state = \<lparr>prod_encode_a = prod_encode_a',
+                       prod_encode_b = prod_encode_b',
+                       prod_encode_ret = prod_encode_ret'\<rparr>;
+   prod_encode_ret_state = prod_encode_imp prod_encode_state;
+   t = t + prod_encode_imp_time 0 prod_encode_state;
+
+   operand_bit_to_var_tail_n' = prod_encode_ret prod_encode_ret_state;
+   t = t + 2;
+   operand_bit_to_var_tail_ret' = 0;
+   t = t + 2;
+   operand_bit_to_var_tail_state = \<lparr>operand_bit_to_var_tail_n = operand_bit_to_var_tail_n',
+                               operand_bit_to_var_tail_ret = operand_bit_to_var_tail_ret'\<rparr>;
+   operand_bit_to_var_tail_ret_state = operand_bit_to_var_tail_imp operand_bit_to_var_tail_state;
+   t = t + operand_bit_to_var_tail_imp_time 0 operand_bit_to_var_tail_state;
+
+   cons_h' = 1;
+   t = t + 2;
+   cons_t' = 0;
+   t = t + 2;
+   cons_ret' = 0;
+   t = t + 2;
+   cons_state = \<lparr>cons_h = cons_h', cons_t = cons_t', cons_ret = cons_ret'\<rparr>;
+   cons_ret_state = cons_imp cons_state;
+   t = t + cons_imp_time 0 cons_state;
+
+   cons_h' = operand_bit_to_var_tail_ret operand_bit_to_var_tail_ret_state;
+   t = t + 2;
+   cons_t' = cons_ret cons_ret_state;
+   t = t + 2;
+   cons_ret' = 0;
+   t = t + 2;
+   cons_state = \<lparr>cons_h = cons_h', cons_t = cons_t', cons_ret = cons_ret'\<rparr>;
+   cons_ret_state = cons_imp cons_state;
+   t = t + cons_imp_time 0 cons_state;
+
+   cons_h' = 1;
+   t = t + 2;
+   cons_t' = cons_ret cons_ret_state;
+   t = t + 2;
+   cons_ret' = 0;
+   t = t + 2;
+   cons_state = \<lparr>cons_h = cons_h', cons_t = cons_t', cons_ret = cons_ret'\<rparr>;
+   cons_ret_state = cons_imp cons_state;
+   t = t + cons_imp_time 0 cons_state;
+
+   copy_var_to_operand_aux2_ret' = cons_ret cons_ret_state;
+   t = t + 2;
+   ret = \<lparr>copy_var_to_operand_aux2_op = copy_var_to_operand_aux2_op s,
+         copy_var_to_operand_aux2_diff = copy_var_to_operand_aux2_diff s,
+         copy_var_to_operand_aux2_ret = copy_var_to_operand_aux2_ret'\<rparr>
+  in
+   t)"
+
+function copy_var_to_operand_aux2_imp_time 
+ :: "nat \<Rightarrow> copy_var_to_operand_aux2_state \<Rightarrow> nat" where 
+"copy_var_to_operand_aux2_imp_time t s = 
+  (let
+     ret = copy_var_to_operand_aux2_imp_state_upd s;
+     t = t + copy_var_to_operand_aux2_imp_state_upd_time 0 s
+   in
+    t)" by auto
+termination 
+  by (relation "measure (copy_var_to_operand_aux2_op \<circ> snd)", simp)
+
+definition "copy_var_to_operand_aux2_IMP_Minus \<equiv> 
+  (prod_encode_prefix @ prod_encode_a_str) ::= A (V copy_var_to_operand_aux2_op_str);;
+  (prod_encode_prefix @ prod_encode_b_str) ::= A (V copy_var_to_operand_aux2_diff_str);;
+  (prod_encode_prefix @ prod_encode_ret_str) ::= A (N 0);;
+  invoke_subprogram prod_encode_prefix prod_encode_IMP_Minus;;
+  
+  (operand_bit_to_var_tail_prefix @ operand_bit_to_var_tail_n_str) ::= A (V (prod_encode_prefix @ prod_encode_ret_str));;
+  (operand_bit_to_var_tail_prefix @ operand_bit_to_var_tail_ret_str) ::= A (N 0);;
+  invoke_subprogram operand_bit_to_var_tail_prefix operand_bit_to_var_tail_IMP_Minus;;
+
+  (cons_prefix @ cons_h_str) ::= A (N 1);;
+  (cons_prefix @ cons_t_str) ::= A (N 0);;
+  (cons_prefix @ cons_ret_str) ::= A (N 0);;
+  invoke_subprogram cons_prefix cons_IMP_Minus;;
+
+  (cons_prefix @ cons_h_str) ::= A (V (operand_bit_to_var_tail_prefix @ operand_bit_to_var_tail_ret_str));;
+  (cons_prefix @ cons_t_str) ::= A (V (cons_prefix @ cons_ret_str));;
+  (cons_prefix @ cons_ret_str) ::= A (N 0);;
+  invoke_subprogram cons_prefix cons_IMP_Minus;;
+
+  (cons_prefix @ cons_h_str) ::= A (N 1);;
+  (cons_prefix @ cons_t_str) ::= A (V (cons_prefix @ cons_ret_str));;
+  (cons_prefix @ cons_ret_str) ::= A (N 0);;
+  invoke_subprogram cons_prefix cons_IMP_Minus;;
+  
+  copy_var_to_operand_aux2_ret_str ::= A (V (cons_prefix @ cons_ret_str))"
+
+abbreviation "copy_var_to_operand_aux2_IMP_vars \<equiv> 
+  {copy_var_to_operand_aux2_op_str, copy_var_to_operand_aux2_diff_str, copy_var_to_operand_aux2_ret_str}"
+
+definition "copy_var_to_operand_aux2_imp_to_HOL_state p s \<equiv> 
+  \<lparr>copy_var_to_operand_aux2_op = s (add_prefix p copy_var_to_operand_aux2_op_str),
+  copy_var_to_operand_aux2_diff = s (add_prefix p copy_var_to_operand_aux2_diff_str),
+  copy_var_to_operand_aux2_ret = s (add_prefix p copy_var_to_operand_aux2_ret_str)\<rparr>"
+
+lemmas copy_var_to_operand_aux2_state_translators =
+  copy_var_to_operand_aux2_imp_to_HOL_state_def
+  cons_imp_to_HOL_state_def
+  operand_bit_to_var_tail_imp_to_HOL_state_def 
+  prod_encode_imp_to_HOL_state_def
+
+lemma copy_var_to_operand_aux2_IMP_Minus_correct_function:
+  "(invoke_subprogram p copy_var_to_operand_aux2_IMP_Minus, s) \<Rightarrow>\<^bsup>t\<^esup> s' \<Longrightarrow>
+     s' (add_prefix p copy_var_to_operand_aux2_ret_str)
+      = copy_var_to_operand_aux2_ret (copy_var_to_operand_aux2_imp (copy_var_to_operand_aux2_imp_to_HOL_state p s))"
+  apply (simp only: copy_var_to_operand_aux2_imp.simps copy_var_to_operand_aux2_imp_state_upd_def)
+  apply (simp only: copy_var_to_operand_aux2_IMP_Minus_def prefix_simps)
+  apply (erule Seq_E)+
+  apply (erule prod_encode_IMP_Minus_correct[where vars=copy_var_to_operand_aux2_IMP_vars])
+  subgoal premises p using p(20) by fastforce
+  apply (erule operand_bit_to_var_tail_IMP_Minus_correct[where vars=copy_var_to_operand_aux2_IMP_vars])
+  subgoal premises p using p(22) by fastforce
+  apply (erule cons_IMP_Minus_correct[where vars=copy_var_to_operand_aux2_IMP_vars])
+  subgoal premises p using p(24) by fastforce
+  apply (erule cons_IMP_Minus_correct[where vars=copy_var_to_operand_aux2_IMP_vars])
+  subgoal premises p using p(26) by fastforce
+  apply (erule cons_IMP_Minus_correct[where vars="copy_var_to_operand_aux2_IMP_vars 
+    \<union> {operand_bit_to_var_tail_prefix @ operand_bit_to_var_tail_ret_str}"])
+  subgoal premises p using p(28) by fastforce
+  apply (force simp: copy_var_to_operand_aux2_state_translators Let_def) 
+  done 
+
+lemma copy_var_to_operand_aux2_IMP_Minus_correct_time:
+  "(invoke_subprogram p copy_var_to_operand_aux2_IMP_Minus, s) \<Rightarrow>\<^bsup>t\<^esup> s' \<Longrightarrow>
+     t = copy_var_to_operand_aux2_imp_time 0 (copy_var_to_operand_aux2_imp_to_HOL_state p s)"
+  apply (simp only: copy_var_to_operand_aux2_imp_time.simps copy_var_to_operand_aux2_imp_state_upd_time_def)
+  apply (simp only: copy_var_to_operand_aux2_IMP_Minus_def prefix_simps)
+  apply (erule Seq_tE)+
+  apply (erule prod_encode_IMP_Minus_correct[where vars=copy_var_to_operand_aux2_IMP_vars])
+  subgoal premises p using p(39) by fastforce
+  apply (erule operand_bit_to_var_tail_IMP_Minus_correct[where vars=copy_var_to_operand_aux2_IMP_vars])
+  subgoal premises p using p(41) by fastforce
+  apply (erule cons_IMP_Minus_correct[where vars=copy_var_to_operand_aux2_IMP_vars])
+  subgoal premises p using p(43) by fastforce
+  apply (erule cons_IMP_Minus_correct[where vars=copy_var_to_operand_aux2_IMP_vars])
+  subgoal premises p using p(45) by fastforce
+  apply (erule cons_IMP_Minus_correct[where vars="copy_var_to_operand_aux2_IMP_vars 
+    \<union> {operand_bit_to_var_tail_prefix @ operand_bit_to_var_tail_ret_str}"])
+  subgoal premises p using p(47) by fastforce
+  apply (force simp: copy_var_to_operand_aux2_state_translators Let_def) 
+  done 
+
+lemma copy_var_to_operand_aux2_IMP_Minus_correct:
+  "\<lbrakk>(invoke_subprogram (p1 @ p2) copy_var_to_operand_aux2_IMP_Minus, s) \<Rightarrow>\<^bsup>t\<^esup> s';
+    \<And>v. v \<in> vars \<Longrightarrow> \<not> (set p2 \<subseteq> set v);
+     \<lbrakk>t = (copy_var_to_operand_aux2_imp_time 0 (copy_var_to_operand_aux2_imp_to_HOL_state (p1 @ p2) s));
+      s' (add_prefix (p1 @ p2) copy_var_to_operand_aux2_ret_str) =
+        copy_var_to_operand_aux2_ret
+          (copy_var_to_operand_aux2_imp (copy_var_to_operand_aux2_imp_to_HOL_state (p1 @ p2) s));
+      \<And>v. v \<in> vars \<Longrightarrow> s (add_prefix p1 v) = s' (add_prefix p1 v)\<rbrakk>
+     \<Longrightarrow> P\<rbrakk> \<Longrightarrow> P"
+  using copy_var_to_operand_aux2_IMP_Minus_correct_function 
+      copy_var_to_operand_aux2_IMP_Minus_correct_time
+       set_mono_prefix
+  by (smt (verit, ccfv_SIG) com_add_prefix_valid_subset com_only_vars)
+
+subsubsection copy_var_to_operand_aux3
+
+record copy_var_to_operand_aux3_state=
+copy_var_to_operand_aux3_op::nat
+copy_var_to_operand_aux3_diff::nat
+copy_var_to_operand_aux3_ret::nat
+
+abbreviation "copy_var_to_operand_aux3_prefix \<equiv> ''copy_var_to_operand_aux3_op.''"
+abbreviation "copy_var_to_operand_aux3_op_str \<equiv> ''op''"
+abbreviation "copy_var_to_operand_aux3_diff_str \<equiv> ''diff''"
+abbreviation "copy_var_to_operand_aux3_ret_str \<equiv> ''ret''"
+
+definition "copy_var_to_operand_aux3_imp_state_upd s \<equiv> 
+ (let
+   prod_encode_a' = copy_var_to_operand_aux3_op s;
+   prod_encode_b' = copy_var_to_operand_aux3_diff s;
+   prod_encode_ret' = 0;
+   prod_encode_state = \<lparr>prod_encode_a = prod_encode_a',
+                       prod_encode_b = prod_encode_b',
+                       prod_encode_ret = prod_encode_ret'\<rparr>;
+   prod_encode_ret_state = prod_encode_imp prod_encode_state;
+   operand_bit_to_var_tail_n' = prod_encode_ret prod_encode_ret_state;
+   operand_bit_to_var_tail_ret' = 0;
+   operand_bit_to_var_tail_state = \<lparr>operand_bit_to_var_tail_n = operand_bit_to_var_tail_n',
+                               operand_bit_to_var_tail_ret = operand_bit_to_var_tail_ret'\<rparr>;
+   operand_bit_to_var_tail_ret_state = operand_bit_to_var_tail_imp operand_bit_to_var_tail_state;
+
+   cons_h' = 0;
+   cons_t' = 0;
+   cons_ret' = 0;
+   cons_state = \<lparr>cons_h = cons_h', cons_t = cons_t', cons_ret = cons_ret'\<rparr>;
+   cons_ret_state = cons_imp cons_state;
+
+   cons_h' = operand_bit_to_var_tail_ret operand_bit_to_var_tail_ret_state;
+   cons_t' = cons_ret cons_ret_state;
+   cons_ret' = 0;
+   cons_state = \<lparr>cons_h = cons_h', cons_t = cons_t', cons_ret = cons_ret'\<rparr>;
+   cons_ret_state = cons_imp cons_state;
+
+   cons_h' = 1;
+   cons_t' = cons_ret cons_ret_state;
+   cons_ret' = 0;
+   cons_state = \<lparr>cons_h = cons_h', cons_t = cons_t', cons_ret = cons_ret'\<rparr>;
+   cons_ret_state = cons_imp cons_state;
+
+   copy_var_to_operand_aux3_ret' = cons_ret cons_ret_state;
+   ret = \<lparr>copy_var_to_operand_aux3_op = copy_var_to_operand_aux3_op s,
+         copy_var_to_operand_aux3_diff = copy_var_to_operand_aux3_diff s,
+         copy_var_to_operand_aux3_ret = copy_var_to_operand_aux3_ret'\<rparr>
+  in
+   ret)"
+
+function copy_var_to_operand_aux3_imp 
+ :: "copy_var_to_operand_aux3_state \<Rightarrow> copy_var_to_operand_aux3_state" where 
+"copy_var_to_operand_aux3_imp s = 
+  (let
+     ret = copy_var_to_operand_aux3_imp_state_upd s
+   in
+    ret)" by simp+
+termination 
+  by (relation "measure copy_var_to_operand_aux3_op", simp)
+
+declare copy_var_to_operand_aux3_imp.simps[simp del]
+
+lemma copy_var_to_operand_aux3_imp_correct[let_function_correctness]:
+  "copy_var_to_operand_aux3_ret (copy_var_to_operand_aux3_imp s)
+    = (1 ## (operand_bit_to_var_tail (prod_encode (
+        (copy_var_to_operand_aux3_op s), (copy_var_to_operand_aux3_diff s)))) ## 0 ## 0)"
+apply (subst copy_var_to_operand_aux3_imp.simps copy_var_to_operand_aux3_imp_state_upd_def)+
+apply (auto simp add: Let_def operand_bit_to_var_tail_imp_correct 
+  cons_imp_correct prod_encode_imp_correct)
+done 
+
+definition "copy_var_to_operand_aux3_imp_state_upd_time t s \<equiv> 
+ (let
+   prod_encode_a' = copy_var_to_operand_aux3_op s;
+   t = t + 2;
+   prod_encode_b' = copy_var_to_operand_aux3_diff s;
+   t = t + 2;
+   prod_encode_ret' = 0;
+   t = t + 2;
+   prod_encode_state = \<lparr>prod_encode_a = prod_encode_a',
+                       prod_encode_b = prod_encode_b',
+                       prod_encode_ret = prod_encode_ret'\<rparr>;
+   prod_encode_ret_state = prod_encode_imp prod_encode_state;
+   t = t + prod_encode_imp_time 0 prod_encode_state;
+
+   operand_bit_to_var_tail_n' = prod_encode_ret prod_encode_ret_state;
+   t = t + 2;
+   operand_bit_to_var_tail_ret' = 0;
+   t = t + 2;
+   operand_bit_to_var_tail_state = \<lparr>operand_bit_to_var_tail_n = operand_bit_to_var_tail_n',
+                               operand_bit_to_var_tail_ret = operand_bit_to_var_tail_ret'\<rparr>;
+   operand_bit_to_var_tail_ret_state = operand_bit_to_var_tail_imp operand_bit_to_var_tail_state;
+   t = t + operand_bit_to_var_tail_imp_time 0 operand_bit_to_var_tail_state;
+
+   cons_h' = 0;
+   t = t + 2;
+   cons_t' = 0;
+   t = t + 2;
+   cons_ret' = 0;
+   t = t + 2;
+   cons_state = \<lparr>cons_h = cons_h', cons_t = cons_t', cons_ret = cons_ret'\<rparr>;
+   cons_ret_state = cons_imp cons_state;
+   t = t + cons_imp_time 0 cons_state;
+
+   cons_h' = operand_bit_to_var_tail_ret operand_bit_to_var_tail_ret_state;
+   t = t + 2;
+   cons_t' = cons_ret cons_ret_state;
+   t = t + 2;
+   cons_ret' = 0;
+   t = t + 2;
+   cons_state = \<lparr>cons_h = cons_h', cons_t = cons_t', cons_ret = cons_ret'\<rparr>;
+   cons_ret_state = cons_imp cons_state;
+   t = t + cons_imp_time 0 cons_state;
+
+   cons_h' = 1;
+   t = t + 2;
+   cons_t' = cons_ret cons_ret_state;
+   t = t + 2;
+   cons_ret' = 0;
+   t = t + 2;
+   cons_state = \<lparr>cons_h = cons_h', cons_t = cons_t', cons_ret = cons_ret'\<rparr>;
+   cons_ret_state = cons_imp cons_state;
+   t = t + cons_imp_time 0 cons_state;
+
+   copy_var_to_operand_aux3_ret' = cons_ret cons_ret_state;
+   t = t + 2;
+   ret = \<lparr>copy_var_to_operand_aux3_op = copy_var_to_operand_aux3_op s,
+         copy_var_to_operand_aux3_diff = copy_var_to_operand_aux3_diff s,
+         copy_var_to_operand_aux3_ret = copy_var_to_operand_aux3_ret'\<rparr>
+  in
+   t)"
+
+function copy_var_to_operand_aux3_imp_time 
+ :: "nat \<Rightarrow> copy_var_to_operand_aux3_state \<Rightarrow> nat" where 
+"copy_var_to_operand_aux3_imp_time t s = 
+  (let
+     ret = copy_var_to_operand_aux3_imp_state_upd s;
+     t = t + copy_var_to_operand_aux3_imp_state_upd_time 0 s
+   in
+    t)" by auto
+termination 
+  by (relation "measure (copy_var_to_operand_aux3_op \<circ> snd)", simp)
+
+definition "copy_var_to_operand_aux3_IMP_Minus \<equiv> 
+  (prod_encode_prefix @ prod_encode_a_str) ::= A (V copy_var_to_operand_aux3_op_str);;
+  (prod_encode_prefix @ prod_encode_b_str) ::= A (V copy_var_to_operand_aux3_diff_str);;
+  (prod_encode_prefix @ prod_encode_ret_str) ::= A (N 0);;
+  invoke_subprogram prod_encode_prefix prod_encode_IMP_Minus;;
+  
+  (operand_bit_to_var_tail_prefix @ operand_bit_to_var_tail_n_str) ::= A (V (prod_encode_prefix @ prod_encode_ret_str));;
+  (operand_bit_to_var_tail_prefix @ operand_bit_to_var_tail_ret_str) ::= A (N 0);;
+  invoke_subprogram operand_bit_to_var_tail_prefix operand_bit_to_var_tail_IMP_Minus;;
+
+  (cons_prefix @ cons_h_str) ::= A (N 0);;
+  (cons_prefix @ cons_t_str) ::= A (N 0);;
+  (cons_prefix @ cons_ret_str) ::= A (N 0);;
+  invoke_subprogram cons_prefix cons_IMP_Minus;;
+
+  (cons_prefix @ cons_h_str) ::= A (V (operand_bit_to_var_tail_prefix @ operand_bit_to_var_tail_ret_str));;
+  (cons_prefix @ cons_t_str) ::= A (V (cons_prefix @ cons_ret_str));;
+  (cons_prefix @ cons_ret_str) ::= A (N 0);;
+  invoke_subprogram cons_prefix cons_IMP_Minus;;
+
+  (cons_prefix @ cons_h_str) ::= A (N 1);;
+  (cons_prefix @ cons_t_str) ::= A (V (cons_prefix @ cons_ret_str));;
+  (cons_prefix @ cons_ret_str) ::= A (N 0);;
+  invoke_subprogram cons_prefix cons_IMP_Minus;;
+  
+  copy_var_to_operand_aux3_ret_str ::= A (V (cons_prefix @ cons_ret_str))"
+
+abbreviation "copy_var_to_operand_aux3_IMP_vars \<equiv> 
+  {copy_var_to_operand_aux3_op_str, copy_var_to_operand_aux3_diff_str, copy_var_to_operand_aux3_ret_str}"
+
+definition "copy_var_to_operand_aux3_imp_to_HOL_state p s \<equiv> 
+  \<lparr>copy_var_to_operand_aux3_op = s (add_prefix p copy_var_to_operand_aux3_op_str),
+  copy_var_to_operand_aux3_diff = s (add_prefix p copy_var_to_operand_aux3_diff_str),
+  copy_var_to_operand_aux3_ret = s (add_prefix p copy_var_to_operand_aux3_ret_str)\<rparr>"
+
+lemmas copy_var_to_operand_aux3_state_translators =
+  copy_var_to_operand_aux3_imp_to_HOL_state_def
+  cons_imp_to_HOL_state_def
+  operand_bit_to_var_tail_imp_to_HOL_state_def 
+  prod_encode_imp_to_HOL_state_def
+
+lemma copy_var_to_operand_aux3_IMP_Minus_correct_function:
+  "(invoke_subprogram p copy_var_to_operand_aux3_IMP_Minus, s) \<Rightarrow>\<^bsup>t\<^esup> s' \<Longrightarrow>
+     s' (add_prefix p copy_var_to_operand_aux3_ret_str)
+      = copy_var_to_operand_aux3_ret (copy_var_to_operand_aux3_imp (copy_var_to_operand_aux3_imp_to_HOL_state p s))"
+  apply (simp only: copy_var_to_operand_aux3_imp.simps copy_var_to_operand_aux3_imp_state_upd_def)
+  apply (simp only: copy_var_to_operand_aux3_IMP_Minus_def prefix_simps)
+  apply (erule Seq_E)+
+  apply (erule prod_encode_IMP_Minus_correct[where vars=copy_var_to_operand_aux3_IMP_vars])
+  subgoal premises p using p(20) by fastforce
+  apply (erule operand_bit_to_var_tail_IMP_Minus_correct[where vars=copy_var_to_operand_aux3_IMP_vars])
+  subgoal premises p using p(22) by fastforce
+  apply (erule cons_IMP_Minus_correct[where vars=copy_var_to_operand_aux3_IMP_vars])
+  subgoal premises p using p(24) by fastforce
+  apply (erule cons_IMP_Minus_correct[where vars=copy_var_to_operand_aux3_IMP_vars])
+  subgoal premises p using p(26) by fastforce
+  apply (erule cons_IMP_Minus_correct[where vars="copy_var_to_operand_aux3_IMP_vars 
+    \<union> {operand_bit_to_var_tail_prefix @ operand_bit_to_var_tail_ret_str}"])
+  subgoal premises p using p(28) by fastforce
+  apply (force simp: copy_var_to_operand_aux3_state_translators Let_def) 
+  done 
+
+lemma copy_var_to_operand_aux3_IMP_Minus_correct_time:
+  "(invoke_subprogram p copy_var_to_operand_aux3_IMP_Minus, s) \<Rightarrow>\<^bsup>t\<^esup> s' \<Longrightarrow>
+     t = copy_var_to_operand_aux3_imp_time 0 (copy_var_to_operand_aux3_imp_to_HOL_state p s)"
+  apply (simp only: copy_var_to_operand_aux3_imp_time.simps copy_var_to_operand_aux3_imp_state_upd_time_def)
+  apply (simp only: copy_var_to_operand_aux3_IMP_Minus_def prefix_simps)
+  apply (erule Seq_tE)+
+  apply (erule prod_encode_IMP_Minus_correct[where vars=copy_var_to_operand_aux3_IMP_vars])
+  subgoal premises p using p(39) by fastforce
+  apply (erule operand_bit_to_var_tail_IMP_Minus_correct[where vars=copy_var_to_operand_aux3_IMP_vars])
+  subgoal premises p using p(41) by fastforce
+  apply (erule cons_IMP_Minus_correct[where vars=copy_var_to_operand_aux3_IMP_vars])
+  subgoal premises p using p(43) by fastforce
+  apply (erule cons_IMP_Minus_correct[where vars=copy_var_to_operand_aux3_IMP_vars])
+  subgoal premises p using p(45) by fastforce
+  apply (erule cons_IMP_Minus_correct[where vars="copy_var_to_operand_aux3_IMP_vars 
+    \<union> {operand_bit_to_var_tail_prefix @ operand_bit_to_var_tail_ret_str}"])
+  subgoal premises p using p(47) by fastforce
+  apply (force simp: copy_var_to_operand_aux3_state_translators Let_def) 
+  done 
+
+lemma copy_var_to_operand_aux3_IMP_Minus_correct:
+  "\<lbrakk>(invoke_subprogram (p1 @ p2) copy_var_to_operand_aux3_IMP_Minus, s) \<Rightarrow>\<^bsup>t\<^esup> s';
+    \<And>v. v \<in> vars \<Longrightarrow> \<not> (set p2 \<subseteq> set v);
+     \<lbrakk>t = (copy_var_to_operand_aux3_imp_time 0 (copy_var_to_operand_aux3_imp_to_HOL_state (p1 @ p2) s));
+      s' (add_prefix (p1 @ p2) copy_var_to_operand_aux3_ret_str) =
+        copy_var_to_operand_aux3_ret
+          (copy_var_to_operand_aux3_imp (copy_var_to_operand_aux3_imp_to_HOL_state (p1 @ p2) s));
+      \<And>v. v \<in> vars \<Longrightarrow> s (add_prefix p1 v) = s' (add_prefix p1 v)\<rbrakk>
+     \<Longrightarrow> P\<rbrakk> \<Longrightarrow> P"
+  using copy_var_to_operand_aux3_IMP_Minus_correct_function 
+      copy_var_to_operand_aux3_IMP_Minus_correct_time
+       set_mono_prefix
+  by (smt (verit, ccfv_SIG) com_add_prefix_valid_subset com_only_vars)
+
+subsubsection copy_var_to_operand_aux4
+
+record copy_var_to_operand_aux4_state=
+  copy_var_to_operand_aux4_diff::nat
+  copy_var_to_operand_aux4_i::nat
+  copy_var_to_operand_aux4_op::nat
+  copy_var_to_operand_aux4_v::nat 
+  copy_var_to_operand_aux4_ret::nat
+
+abbreviation "copy_var_to_operand_aux4_prefix \<equiv> ''copy_var_to_operand_aux4_prefix.''"
+abbreviation "copy_var_to_operand_aux4_diff_str \<equiv> ''diff''"
+abbreviation "copy_var_to_operand_aux4_i_str \<equiv> ''i''"
+abbreviation "copy_var_to_operand_aux4_op_str \<equiv> ''op''"
+abbreviation "copy_var_to_operand_aux4_v_str \<equiv> ''v''"
+abbreviation "copy_var_to_operand_aux4_ret_str \<equiv> ''ret''"
+
+definition "copy_var_to_operand_aux4_state_upd s \<equiv> 
+ (let
+   copy_var_to_operand_aux3_op' = copy_var_to_operand_aux4_op s;
+   copy_var_to_operand_aux3_diff' = copy_var_to_operand_aux4_i s - copy_var_to_operand_aux4_diff s;
+   copy_var_to_operand_aux3_ret' = 0;
+   copy_var_to_operand_aux3_state = \<lparr>copy_var_to_operand_aux3_op = copy_var_to_operand_aux3_op',
+                                    copy_var_to_operand_aux3_diff = copy_var_to_operand_aux3_diff',
+                                    copy_var_to_operand_aux3_ret = copy_var_to_operand_aux3_ret'\<rparr>;
+   copy_var_to_operand_aux3_ret_state = copy_var_to_operand_aux3_imp copy_var_to_operand_aux3_state;
+
+   cons_h' = copy_var_to_operand_aux3_ret copy_var_to_operand_aux3_ret_state;
+   cons_t' = 0;
+   cons_ret' = 0;
+   cons_state = \<lparr>cons_h = cons_h', cons_t = cons_t', cons_ret = cons_ret'\<rparr>;
+   cons_ret_state = cons_imp cons_state;
+
+   copy_var_to_operand_aux2_op' = copy_var_to_operand_aux4_op s;
+   copy_var_to_operand_aux2_diff' = copy_var_to_operand_aux4_i s - copy_var_to_operand_aux4_diff s;
+   copy_var_to_operand_aux2_ret' = 0;
+   copy_var_to_operand_aux2_state = \<lparr>copy_var_to_operand_aux2_op = copy_var_to_operand_aux2_op',
+                                    copy_var_to_operand_aux2_diff = copy_var_to_operand_aux2_diff',
+                                    copy_var_to_operand_aux2_ret = copy_var_to_operand_aux2_ret'\<rparr>;
+   copy_var_to_operand_aux2_ret_state = copy_var_to_operand_aux2_imp copy_var_to_operand_aux2_state;
+
+   cons_h' = copy_var_to_operand_aux2_ret copy_var_to_operand_aux2_ret_state;
+   cons_t' = cons_ret cons_ret_state;
+   cons_ret' = 0;
+   cons_state = \<lparr>cons_h = cons_h', cons_t = cons_t', cons_ret = cons_ret'\<rparr>;
+   cons_ret_state = cons_imp cons_state;
+
+   copy_var_to_operand_aux1_op' = copy_var_to_operand_aux4_v s;
+   copy_var_to_operand_aux1_diff' = copy_var_to_operand_aux4_i s - copy_var_to_operand_aux4_diff s;
+   copy_var_to_operand_aux1_ret' = 0;
+   copy_var_to_operand_aux1_state = \<lparr>copy_var_to_operand_aux1_op = copy_var_to_operand_aux1_op',
+                                    copy_var_to_operand_aux1_diff = copy_var_to_operand_aux1_diff',
+                                    copy_var_to_operand_aux1_ret = copy_var_to_operand_aux1_ret'\<rparr>;
+  copy_var_to_operand_aux1_ret_state = copy_var_to_operand_aux1_imp copy_var_to_operand_aux1_state;
+
+ cons_h' = copy_var_to_operand_aux1_ret copy_var_to_operand_aux1_ret_state;
+ cons_t' = cons_ret cons_ret_state; 
+ cons_ret' = 0;
+ cons_state = \<lparr>cons_h = cons_h', cons_t = cons_t', cons_ret = cons_ret'\<rparr>;
+ cons_ret_state = cons_imp cons_state;
+
+ cons_h' = 3;
+ cons_t' = cons_ret cons_ret_state; 
+ cons_ret' = 0;
+ cons_state = \<lparr>cons_h = cons_h', cons_t = cons_t', cons_ret = cons_ret'\<rparr>;
+ cons_ret_state = cons_imp cons_state;
+
+ copy_var_to_operand_aux4_ret' = cons_ret cons_ret_state;
+ ret = \<lparr>copy_var_to_operand_aux4_diff = copy_var_to_operand_aux4_diff s,
+       copy_var_to_operand_aux4_i = copy_var_to_operand_aux4_i s,
+       copy_var_to_operand_aux4_op = copy_var_to_operand_aux4_op s,
+       copy_var_to_operand_aux4_v = copy_var_to_operand_aux4_v s,
+       copy_var_to_operand_aux4_ret = copy_var_to_operand_aux4_ret'\<rparr>
+ in
+  ret)"
+
+function copy_var_to_operand_aux4_imp 
+  :: "copy_var_to_operand_aux4_state \<Rightarrow> copy_var_to_operand_aux4_state" where
+"copy_var_to_operand_aux4_imp s = 
+  (let
+    ret = copy_var_to_operand_aux4_state_upd s
+   in
+    ret)" by simp+
+termination 
+ by (relation "measure copy_var_to_operand_aux4_diff", simp)
+
+declare copy_var_to_operand_aux4_imp.simps[simp del]
+
+lemma copy_var_to_operand_aux4_imp_correct:
+  "copy_var_to_operand_aux4_ret (copy_var_to_operand_aux4_imp s) = 
+    (3 ## ((var_bit_to_var_tail (prod_encode ((copy_var_to_operand_aux4_v s), 
+      (copy_var_to_operand_aux4_i s) - (copy_var_to_operand_aux4_diff s)))) ## 0)
+    ## (1 ## (operand_bit_to_var_tail (prod_encode ((copy_var_to_operand_aux4_op s), 
+       (copy_var_to_operand_aux4_i s) - (copy_var_to_operand_aux4_diff s)))) ## 1 ## 0)
+    ## (1 ## (operand_bit_to_var_tail (prod_encode ((copy_var_to_operand_aux4_op s), 
+      (copy_var_to_operand_aux4_i s) - (copy_var_to_operand_aux4_diff s)))) ## 0 ## 0)
+    ## 0)"
+  apply (simp only: copy_var_to_operand_aux4_imp.simps copy_var_to_operand_aux4_state_upd_def)
+  apply (auto simp add: cons_imp_correct Let_def 
+    copy_var_to_operand_aux1_imp_correct copy_var_to_operand_aux3_imp_correct
+    copy_var_to_operand_aux2_imp_correct)
+  done 
+
+definition "copy_var_to_operand_aux4_state_upd_time t s \<equiv> 
+ (let
+   copy_var_to_operand_aux3_op' = copy_var_to_operand_aux4_op s;
+   t = t + 2;
+   copy_var_to_operand_aux3_diff' = copy_var_to_operand_aux4_i s - copy_var_to_operand_aux4_diff s;
+   t = t + 2;
+   copy_var_to_operand_aux3_ret' = 0;
+   t = t + 2;
+   copy_var_to_operand_aux3_state = \<lparr>copy_var_to_operand_aux3_op = copy_var_to_operand_aux3_op',
+                                    copy_var_to_operand_aux3_diff = copy_var_to_operand_aux3_diff',
+                                    copy_var_to_operand_aux3_ret = copy_var_to_operand_aux3_ret'\<rparr>;
+   copy_var_to_operand_aux3_ret_state = copy_var_to_operand_aux3_imp copy_var_to_operand_aux3_state;
+   t = t + copy_var_to_operand_aux3_imp_time 0 copy_var_to_operand_aux3_state;
+
+   cons_h' = copy_var_to_operand_aux3_ret copy_var_to_operand_aux3_ret_state;
+   t = t + 2;
+   cons_t' = 0;
+   t = t + 2;
+   cons_ret' = 0;
+   t = t + 2;
+   cons_state = \<lparr>cons_h = cons_h', cons_t = cons_t', cons_ret = cons_ret'\<rparr>;
+   cons_ret_state = cons_imp cons_state;
+   t = t + cons_imp_time 0 cons_state;
+
+   copy_var_to_operand_aux2_op' = copy_var_to_operand_aux4_op s;
+   t = t + 2;
+   copy_var_to_operand_aux2_diff' = copy_var_to_operand_aux4_i s - copy_var_to_operand_aux4_diff s;
+   t = t + 2;
+   copy_var_to_operand_aux2_ret' = 0;
+   t = t + 2;
+   copy_var_to_operand_aux2_state = \<lparr>copy_var_to_operand_aux2_op = copy_var_to_operand_aux2_op',
+                                    copy_var_to_operand_aux2_diff = copy_var_to_operand_aux2_diff',
+                                    copy_var_to_operand_aux2_ret = copy_var_to_operand_aux2_ret'\<rparr>;
+   copy_var_to_operand_aux2_ret_state = copy_var_to_operand_aux2_imp copy_var_to_operand_aux2_state;
+   t = t + copy_var_to_operand_aux2_imp_time 0 copy_var_to_operand_aux2_state;
+
+   cons_h' = copy_var_to_operand_aux2_ret copy_var_to_operand_aux2_ret_state;
+   t = t + 2;
+   cons_t' = cons_ret cons_ret_state;
+   t = t + 2;
+   cons_ret' = 0;
+   t = t + 2;
+   cons_state = \<lparr>cons_h = cons_h', cons_t = cons_t', cons_ret = cons_ret'\<rparr>;
+   cons_ret_state = cons_imp cons_state;
+   t = t + cons_imp_time 0 cons_state;
+
+   copy_var_to_operand_aux1_op' = copy_var_to_operand_aux4_v s;
+   t = t + 2;
+   copy_var_to_operand_aux1_diff' = copy_var_to_operand_aux4_i s - copy_var_to_operand_aux4_diff s;
+   t = t + 2;
+   copy_var_to_operand_aux1_ret' = 0;
+   t = t + 2;
+   copy_var_to_operand_aux1_state = \<lparr>copy_var_to_operand_aux1_op = copy_var_to_operand_aux1_op',
+                                    copy_var_to_operand_aux1_diff = copy_var_to_operand_aux1_diff',
+                                    copy_var_to_operand_aux1_ret = copy_var_to_operand_aux1_ret'\<rparr>;
+  copy_var_to_operand_aux1_ret_state = copy_var_to_operand_aux1_imp copy_var_to_operand_aux1_state;
+   t = t + copy_var_to_operand_aux1_imp_time 0 copy_var_to_operand_aux1_state;
+
+ cons_h' = copy_var_to_operand_aux1_ret copy_var_to_operand_aux1_ret_state;
+   t = t + 2;
+ cons_t' = cons_ret cons_ret_state; 
+   t = t + 2;
+ cons_ret' = 0;
+   t = t + 2;
+ cons_state = \<lparr>cons_h = cons_h', cons_t = cons_t', cons_ret = cons_ret'\<rparr>;
+ cons_ret_state = cons_imp cons_state;
+   t = t + cons_imp_time 0 cons_state;
+
+ cons_h' = 3;
+   t = t + 2;
+ cons_t' = cons_ret cons_ret_state; 
+   t = t + 2;
+ cons_ret' = 0;
+   t = t + 2;
+ cons_state = \<lparr>cons_h = cons_h', cons_t = cons_t', cons_ret = cons_ret'\<rparr>;
+ cons_ret_state = cons_imp cons_state;
+   t = t + cons_imp_time 0 cons_state;
+
+ copy_var_to_operand_aux4_ret' = cons_ret cons_ret_state;
+   t = t + 2;
+ ret = \<lparr>copy_var_to_operand_aux4_diff = copy_var_to_operand_aux4_diff s,
+       copy_var_to_operand_aux4_i = copy_var_to_operand_aux4_i s,
+       copy_var_to_operand_aux4_op = copy_var_to_operand_aux4_op s,
+       copy_var_to_operand_aux4_v = copy_var_to_operand_aux4_v s,
+       copy_var_to_operand_aux4_ret = copy_var_to_operand_aux4_ret'\<rparr>
+ in
+  t)"
+
+
+function copy_var_to_operand_aux4_imp_time 
+  :: "nat \<Rightarrow> copy_var_to_operand_aux4_state \<Rightarrow> nat" where
+"copy_var_to_operand_aux4_imp_time t s = 
+  (let
+    ret = copy_var_to_operand_aux4_state_upd s;
+    t = t + copy_var_to_operand_aux4_state_upd_time 0 s
+   in
+    t)" by auto
+termination 
+ by (relation "measure (copy_var_to_operand_aux4_diff \<circ> snd)", simp)
+
+declare copy_var_to_operand_aux4_imp_time.simps[simp del]
+
+definition "copy_var_to_operand_aux4_IMP_Minus \<equiv> 
+  (copy_var_to_operand_aux3_prefix @ copy_var_to_operand_aux3_op_str)
+    ::= A (V copy_var_to_operand_aux4_op_str);;
+  (copy_var_to_operand_aux3_prefix @ copy_var_to_operand_aux3_diff_str)
+    ::= Sub (V copy_var_to_operand_aux4_i_str) ((V copy_var_to_operand_aux4_diff_str));;
+  (copy_var_to_operand_aux3_prefix @ copy_var_to_operand_aux3_ret_str)
+    ::= A (N 0);;
+  invoke_subprogram copy_var_to_operand_aux3_prefix copy_var_to_operand_aux3_IMP_Minus;;
+  
+  (cons_prefix @ cons_h_str) ::= A (V (copy_var_to_operand_aux3_prefix @ copy_var_to_operand_aux3_ret_str));;
+  (cons_prefix @ cons_t_str) ::= A (N 0);;
+  (cons_prefix @ cons_ret_str) ::= A (N 0);;
+  invoke_subprogram cons_prefix cons_IMP_Minus;;
+
+  (copy_var_to_operand_aux2_prefix @ copy_var_to_operand_aux2_op_str)
+    ::= A (V copy_var_to_operand_aux4_op_str);;
+  (copy_var_to_operand_aux2_prefix @ copy_var_to_operand_aux2_diff_str)
+    ::= Sub (V copy_var_to_operand_aux4_i_str) ((V copy_var_to_operand_aux4_diff_str));;
+  (copy_var_to_operand_aux2_prefix @ copy_var_to_operand_aux2_ret_str)
+    ::= A (N 0);;
+  invoke_subprogram copy_var_to_operand_aux2_prefix copy_var_to_operand_aux2_IMP_Minus;;
+  
+  (cons_prefix @ cons_h_str) ::= A (V (copy_var_to_operand_aux2_prefix @ copy_var_to_operand_aux2_ret_str));;
+  (cons_prefix @ cons_t_str) ::= A (V (cons_prefix @ cons_ret_str));;
+  (cons_prefix @ cons_ret_str) ::= A (N 0);;
+  invoke_subprogram cons_prefix cons_IMP_Minus;;
+  
+  (copy_var_to_operand_aux1_prefix @ copy_var_to_operand_aux1_op_str)
+    ::= A (V copy_var_to_operand_aux4_v_str);;
+  (copy_var_to_operand_aux1_prefix @ copy_var_to_operand_aux1_diff_str)
+    ::= Sub (V copy_var_to_operand_aux4_i_str) ((V copy_var_to_operand_aux4_diff_str));;
+  (copy_var_to_operand_aux1_prefix @ copy_var_to_operand_aux1_ret_str)
+    ::= A (N 0);;
+  invoke_subprogram copy_var_to_operand_aux1_prefix copy_var_to_operand_aux1_IMP_Minus;;
+  
+  (cons_prefix @ cons_h_str) ::= A (V (copy_var_to_operand_aux1_prefix @ copy_var_to_operand_aux1_ret_str));;
+  (cons_prefix @ cons_t_str) ::= A (V (cons_prefix @ cons_ret_str));;
+  (cons_prefix @ cons_ret_str) ::= A (N 0);;
+  invoke_subprogram cons_prefix cons_IMP_Minus;;
+  
+  (cons_prefix @ cons_h_str) ::= A (N 3);;
+  (cons_prefix @ cons_t_str) ::= A (V (cons_prefix @ cons_ret_str));;
+  (cons_prefix @ cons_ret_str) ::= A (N 0);;
+  invoke_subprogram cons_prefix cons_IMP_Minus;;
+  
+  copy_var_to_operand_aux4_ret_str ::= A (V (cons_prefix @ cons_ret_str))"
+
+abbreviation "copy_var_to_operand_aux4_IMP_vars \<equiv> 
+ {copy_var_to_operand_aux4_diff_str, copy_var_to_operand_aux4_i_str,
+ copy_var_to_operand_aux4_op_str, copy_var_to_operand_aux4_v_str}"
+
+definition "copy_var_to_operand_aux4_imp_to_HOL_state p s = 
+  \<lparr>copy_var_to_operand_aux4_diff = s (add_prefix p copy_var_to_operand_aux4_diff_str),
+  copy_var_to_operand_aux4_i = s (add_prefix p copy_var_to_operand_aux4_i_str),
+  copy_var_to_operand_aux4_op = s (add_prefix p copy_var_to_operand_aux4_op_str),
+  copy_var_to_operand_aux4_v = s (add_prefix p copy_var_to_operand_aux4_v_str),
+  copy_var_to_operand_aux4_ret = s (add_prefix p copy_var_to_operand_aux4_ret_str)\<rparr>"
+
+lemmas copy_var_to_operand_aux4_state_translators = 
+  copy_var_to_operand_aux4_imp_to_HOL_state_def
+  copy_var_to_operand_aux3_imp_to_HOL_state_def
+  copy_var_to_operand_aux2_imp_to_HOL_state_def 
+  copy_var_to_operand_aux1_imp_to_HOL_state_def
+  cons_imp_to_HOL_state_def
+    
+lemma copy_var_to_operand_aux4_IMP_Minus_correct_function:
+ "(invoke_subprogram p copy_var_to_operand_aux4_IMP_Minus, s) \<Rightarrow>\<^bsup>t\<^esup> s' \<Longrightarrow>
+     s' (add_prefix p copy_var_to_operand_aux4_ret_str)
+      = copy_var_to_operand_aux4_ret (copy_var_to_operand_aux4_imp (copy_var_to_operand_aux4_imp_to_HOL_state p s))" 
+  apply (simp only: copy_var_to_operand_aux4_imp.simps copy_var_to_operand_aux4_state_upd_def)
+  apply (simp only: copy_var_to_operand_aux4_IMP_Minus_def prefix_simps)  
+  apply (erule Seq_E)+
+  apply (erule copy_var_to_operand_aux3_IMP_Minus_correct[where vars=copy_var_to_operand_aux4_IMP_vars])
+  subgoal premises p using p(29) by fastforce
+  apply (erule cons_IMP_Minus_correct[where vars=copy_var_to_operand_aux4_IMP_vars])
+  subgoal premises p using p(31) by fastforce
+  apply (erule copy_var_to_operand_aux2_IMP_Minus_correct[where vars="copy_var_to_operand_aux4_IMP_vars \<union> {(cons_prefix @ cons_ret_str)}"])
+  subgoal premises p using p(33) by fastforce
+  apply (erule cons_IMP_Minus_correct[where vars=copy_var_to_operand_aux4_IMP_vars])
+  subgoal premises p using p(35) by fastforce
+  apply (erule copy_var_to_operand_aux1_IMP_Minus_correct[where vars="copy_var_to_operand_aux4_IMP_vars \<union> {(cons_prefix @ cons_ret_str)}"])
+  subgoal premises p using p(37) by fastforce
+  apply (erule cons_IMP_Minus_correct[where vars=copy_var_to_operand_aux4_IMP_vars])
+  subgoal premises p using p(39) by fastforce
+  apply (erule cons_IMP_Minus_correct[where vars=copy_var_to_operand_aux4_IMP_vars])
+  subgoal premises p using p(41) by fastforce
+  apply (force simp: copy_var_to_operand_aux4_state_translators Let_def)
+  done
+
+lemma copy_var_to_operand_aux4_IMP_Minus_correct_time:
+ "(invoke_subprogram p copy_var_to_operand_aux4_IMP_Minus, s) \<Rightarrow>\<^bsup>t\<^esup> s' \<Longrightarrow>
+     t = copy_var_to_operand_aux4_imp_time 0 (copy_var_to_operand_aux4_imp_to_HOL_state p s)" 
+  apply (simp only: copy_var_to_operand_aux4_imp_time.simps copy_var_to_operand_aux4_state_upd_time_def)
+  apply (simp only: copy_var_to_operand_aux4_IMP_Minus_def prefix_simps)  
+  apply (erule Seq_tE)+
+  apply (erule copy_var_to_operand_aux3_IMP_Minus_correct[where vars=copy_var_to_operand_aux4_IMP_vars])
+  subgoal premises p using p(57) by fastforce
+  apply (erule cons_IMP_Minus_correct[where vars=copy_var_to_operand_aux4_IMP_vars])
+  subgoal premises p using p(59) by fastforce
+  apply (erule copy_var_to_operand_aux2_IMP_Minus_correct[where vars="copy_var_to_operand_aux4_IMP_vars \<union> {(cons_prefix @ cons_ret_str)}"])
+  subgoal premises p using p(61) by fastforce
+  apply (erule cons_IMP_Minus_correct[where vars=copy_var_to_operand_aux4_IMP_vars])
+  subgoal premises p using p(63) by fastforce
+  apply (erule copy_var_to_operand_aux1_IMP_Minus_correct[where vars="copy_var_to_operand_aux4_IMP_vars \<union> {(cons_prefix @ cons_ret_str)}"])
+  subgoal premises p using p(65) by fastforce
+  apply (erule cons_IMP_Minus_correct[where vars=copy_var_to_operand_aux4_IMP_vars])
+  subgoal premises p using p(67) by fastforce
+  apply (erule cons_IMP_Minus_correct[where vars=copy_var_to_operand_aux4_IMP_vars])
+  subgoal premises p using p(69) by fastforce
+  apply (force simp: copy_var_to_operand_aux4_state_translators Let_def)
+  done
+
+lemma copy_var_to_operand_aux4_IMP_Minus_correct:
+  "\<lbrakk>(invoke_subprogram (p1 @ p2) copy_var_to_operand_aux4_IMP_Minus, s) \<Rightarrow>\<^bsup>t\<^esup> s';
+    \<And>v. v \<in> vars \<Longrightarrow> \<not> (set p2 \<subseteq> set v);
+     \<lbrakk>t = (copy_var_to_operand_aux4_imp_time 0 (copy_var_to_operand_aux4_imp_to_HOL_state (p1 @ p2) s));
+      s' (add_prefix (p1 @ p2) copy_var_to_operand_aux4_ret_str) =
+        copy_var_to_operand_aux4_ret
+          (copy_var_to_operand_aux4_imp (copy_var_to_operand_aux4_imp_to_HOL_state (p1 @ p2) s));
+      \<And>v. v \<in> vars \<Longrightarrow> s (add_prefix p1 v) = s' (add_prefix p1 v)\<rbrakk>
+     \<Longrightarrow> P\<rbrakk> \<Longrightarrow> P"
+  using copy_var_to_operand_aux4_IMP_Minus_correct_function 
+      copy_var_to_operand_aux4_IMP_Minus_correct_time
+       set_mono_prefix
+  by (smt (verit, ccfv_SIG) com_add_prefix_valid_subset com_only_vars)
+
+subsubsection copy_var_to_operand_aux5
+
+record copy_var_to_operand_aux5_state = 
+  copy_var_to_operand_aux5_acc::nat
+  copy_var_to_operand_aux5_diff::nat
+  copy_var_to_operand_aux5_i::nat
+  copy_var_to_operand_aux5_op::nat
+  copy_var_to_operand_aux5_v::nat 
+  copy_var_to_operand_aux5_ret::nat
+
+abbreviation "copy_var_to_operand_aux5_prefix \<equiv> ''copy_var_to_operand_aux5.''"
+abbreviation "copy_var_to_operand_aux5_acc_str \<equiv> ''acc''"
+abbreviation "copy_var_to_operand_aux5_diff_str \<equiv> ''diff''"
+abbreviation "copy_var_to_operand_aux5_i_str \<equiv> ''i''"
+abbreviation "copy_var_to_operand_aux5_op_str \<equiv> ''op''"
+abbreviation "copy_var_to_operand_aux5_v_str \<equiv> ''v''"
+abbreviation "copy_var_to_operand_aux5_ret_str \<equiv> ''ret''"
+
+definition "copy_var_to_operand_aux5_state_upd s \<equiv>
+  (let
+   cons_h' = copy_var_to_operand_aux5_acc s;
+   cons_t' = 0;
+   cons_ret' = 0;
+   cons_state = \<lparr>cons_h = cons_h', cons_t = cons_t', cons_ret = cons_ret'\<rparr>;
+   cons_ret_state = cons_imp cons_state;
+
+   copy_var_to_operand_aux4_diff' = copy_var_to_operand_aux5_diff s;
+   copy_var_to_operand_aux4_i' = copy_var_to_operand_aux5_i s;
+   copy_var_to_operand_aux4_op' = copy_var_to_operand_aux5_op s;
+   copy_var_to_operand_aux4_v' = copy_var_to_operand_aux5_v s;
+   copy_var_to_operand_aux4_ret' = 0;
+   copy_var_to_operand_aux4_state = 
+    \<lparr>copy_var_to_operand_aux4_diff = copy_var_to_operand_aux4_diff',
+    copy_var_to_operand_aux4_i = copy_var_to_operand_aux4_i',
+    copy_var_to_operand_aux4_op = copy_var_to_operand_aux4_op',
+    copy_var_to_operand_aux4_v = copy_var_to_operand_aux4_v',
+    copy_var_to_operand_aux4_ret = copy_var_to_operand_aux4_ret'\<rparr>;
+  copy_var_to_operand_aux4_ret_state = copy_var_to_operand_aux4_imp copy_var_to_operand_aux4_state;
+
+  cons_h' = copy_var_to_operand_aux4_ret copy_var_to_operand_aux4_ret_state;
+  cons_t' = cons_ret cons_ret_state;
+  cons_ret' = 0;
+  cons_state = \<lparr>cons_h = cons_h', cons_t = cons_t', cons_ret = cons_ret'\<rparr>;
+  cons_ret_state = cons_imp cons_state;
+
+  cons_h' = 2;
+  cons_t' = cons_ret cons_ret_state;
+  cons_ret' = 0;
+  cons_state = \<lparr>cons_h = cons_h', cons_t = cons_t', cons_ret = cons_ret'\<rparr>;
+  cons_ret_state = cons_imp cons_state;
+
+  copy_var_to_operand_aux5_ret' = cons_ret cons_ret_state;
+  ret = \<lparr>copy_var_to_operand_aux5_acc = copy_var_to_operand_aux5_acc s,
+        copy_var_to_operand_aux5_diff = copy_var_to_operand_aux5_diff s,
+        copy_var_to_operand_aux5_i = copy_var_to_operand_aux5_i s,
+        copy_var_to_operand_aux5_op = copy_var_to_operand_aux5_op s,
+        copy_var_to_operand_aux5_v = copy_var_to_operand_aux5_v s,
+        copy_var_to_operand_aux5_ret = copy_var_to_operand_aux5_ret'\<rparr>
+  in
+   ret)"
+
+function copy_var_to_operand_aux5_imp :: 
+  "copy_var_to_operand_aux5_state \<Rightarrow> copy_var_to_operand_aux5_state" where
+"copy_var_to_operand_aux5_imp s = 
+  (let
+   ret =copy_var_to_operand_aux5_state_upd s
+  in
+   ret)" by simp+
+  termination 
+   by (relation "measure copy_var_to_operand_aux5_diff", simp)
+
+declare copy_var_to_operand_aux5_imp.simps[simp del]
+
+fun copy_var_to_operand_aux5 :: "nat \<Rightarrow> nat \<Rightarrow> nat \<Rightarrow> nat \<Rightarrow> nat \<Rightarrow> nat" where 
+"copy_var_to_operand_aux5 acc diff i op v = 
+  (2 ## 
+      (3 ## ((var_bit_to_var_tail (prod_encode (v, i - diff))) ## 0)
+          ## (1 ## (operand_bit_to_var_tail (prod_encode (op, i - diff))) ## 1 ## 0)
+          ## (1 ## (operand_bit_to_var_tail (prod_encode (op, i - diff))) ## 0 ## 0)
+          ## 0)
+        ## acc
+        ## 0)"
+
+lemma copy_var_to_operand_aux5_imp_correct:
+  "copy_var_to_operand_aux5_ret (copy_var_to_operand_aux5_imp s) = 
+    copy_var_to_operand_aux5 (copy_var_to_operand_aux5_acc s) (copy_var_to_operand_aux5_diff s)
+     (copy_var_to_operand_aux5_i s) (copy_var_to_operand_aux5_op s) (copy_var_to_operand_aux5_v s)"
+apply (subst copy_var_to_operand_aux5_imp.simps copy_var_to_operand_aux5_state_upd_def)+
+apply (auto simp add: copy_var_to_operand_aux4_imp_correct cons_imp_correct Let_def)
+done 
+
+definition "copy_var_to_operand_aux5_state_upd_time t s \<equiv>
+  (let
+   cons_h' = copy_var_to_operand_aux5_acc s;
+   t = t + 2;
+   cons_t' = 0;
+   t = t + 2;
+   cons_ret' = 0;
+   t = t + 2;
+   cons_state = \<lparr>cons_h = cons_h', cons_t = cons_t', cons_ret = cons_ret'\<rparr>;
+   cons_ret_state = cons_imp cons_state;
+   t = t + cons_imp_time 0 cons_state;
+
+   copy_var_to_operand_aux4_diff' = copy_var_to_operand_aux5_diff s;
+   t = t + 2;
+   copy_var_to_operand_aux4_i' = copy_var_to_operand_aux5_i s;
+   t = t + 2;
+   copy_var_to_operand_aux4_op' = copy_var_to_operand_aux5_op s;
+   t = t + 2;
+   copy_var_to_operand_aux4_v' = copy_var_to_operand_aux5_v s;
+   t = t + 2;
+   copy_var_to_operand_aux4_ret' = 0;
+   t = t + 2;
+   copy_var_to_operand_aux4_state = 
+    \<lparr>copy_var_to_operand_aux4_diff = copy_var_to_operand_aux4_diff',
+    copy_var_to_operand_aux4_i = copy_var_to_operand_aux4_i',
+    copy_var_to_operand_aux4_op = copy_var_to_operand_aux4_op',
+    copy_var_to_operand_aux4_v = copy_var_to_operand_aux4_v',
+    copy_var_to_operand_aux4_ret = copy_var_to_operand_aux4_ret'\<rparr>;
+  copy_var_to_operand_aux4_ret_state = copy_var_to_operand_aux4_imp copy_var_to_operand_aux4_state;
+   t = t + copy_var_to_operand_aux4_imp_time 0 copy_var_to_operand_aux4_state;
+
+  cons_h' = copy_var_to_operand_aux4_ret copy_var_to_operand_aux4_ret_state;
+   t = t + 2;
+  cons_t' = cons_ret cons_ret_state;
+   t = t + 2;
+  cons_ret' = 0;
+   t = t + 2;
+  cons_state = \<lparr>cons_h = cons_h', cons_t = cons_t', cons_ret = cons_ret'\<rparr>;
+  cons_ret_state = cons_imp cons_state;
+   t = t + cons_imp_time 0 cons_state;
+
+  cons_h' = 2;
+   t = t + 2;
+  cons_t' = cons_ret cons_ret_state;
+   t = t + 2;
+  cons_ret' = 0;
+   t = t + 2;
+  cons_state = \<lparr>cons_h = cons_h', cons_t = cons_t', cons_ret = cons_ret'\<rparr>;
+  cons_ret_state = cons_imp cons_state;
+   t = t + cons_imp_time 0 cons_state;
+
+  copy_var_to_operand_aux5_ret' = cons_ret cons_ret_state;
+   t = t + 2;
+  ret = \<lparr>copy_var_to_operand_aux5_acc = copy_var_to_operand_aux5_acc s,
+        copy_var_to_operand_aux5_diff = copy_var_to_operand_aux5_diff s,
+        copy_var_to_operand_aux5_i = copy_var_to_operand_aux5_i s,
+        copy_var_to_operand_aux5_op = copy_var_to_operand_aux5_op s,
+        copy_var_to_operand_aux5_v = copy_var_to_operand_aux5_v s,
+        copy_var_to_operand_aux5_ret = copy_var_to_operand_aux5_ret'\<rparr>
+  in
+   t)"
+
+function copy_var_to_operand_aux5_imp_time :: 
+  "nat \<Rightarrow> copy_var_to_operand_aux5_state \<Rightarrow> nat" where
+"copy_var_to_operand_aux5_imp_time t s = 
+  (let
+   ret =copy_var_to_operand_aux5_state_upd s;
+   t = t + copy_var_to_operand_aux5_state_upd_time 0 s
+  in
+   t)" by auto
+  termination 
+   by (relation "measure (copy_var_to_operand_aux5_diff \<circ> snd)", simp)
+
+declare copy_var_to_operand_aux5_imp_time.simps[simp del]
+
+definition "copy_var_to_operand_aux5_IMP_Minus \<equiv>
+  (cons_prefix @ cons_h_str) ::= A (V copy_var_to_operand_aux5_acc_str);;
+  (cons_prefix @ cons_t_str) ::= A (N 0);;
+  (cons_prefix @ cons_ret_str) ::= A (N 0);;
+  invoke_subprogram cons_prefix cons_IMP_Minus;;
+
+  (copy_var_to_operand_aux4_prefix @ copy_var_to_operand_aux4_diff_str) 
+    ::= A (V (copy_var_to_operand_aux5_diff_str));;
+  (copy_var_to_operand_aux4_prefix @ copy_var_to_operand_aux4_i_str) 
+    ::= A (V copy_var_to_operand_aux5_i_str);;
+  (copy_var_to_operand_aux4_prefix @ copy_var_to_operand_aux4_op_str) 
+    ::= A (V copy_var_to_operand_aux5_op_str);;
+  (copy_var_to_operand_aux4_prefix @ copy_var_to_operand_aux4_v_str) 
+    ::= A (V copy_var_to_operand_aux5_v_str);;
+  (copy_var_to_operand_aux4_prefix @ copy_var_to_operand_aux4_ret_str) 
+    ::= A (N 0);;
+  invoke_subprogram copy_var_to_operand_aux4_prefix copy_var_to_operand_aux4_IMP_Minus;;
+
+  (cons_prefix @ cons_h_str) ::= A (V (copy_var_to_operand_aux4_prefix @ copy_var_to_operand_aux4_ret_str));;
+  (cons_prefix @ cons_t_str) ::= A (V (cons_prefix @ cons_ret_str));;
+  (cons_prefix @ cons_ret_str) ::= A (N 0);;
+  invoke_subprogram cons_prefix cons_IMP_Minus;;
+
+  (cons_prefix @ cons_h_str) ::= A (N 2);;
+  (cons_prefix @ cons_t_str) ::= A (V (cons_prefix @ cons_ret_str));;
+  (cons_prefix @ cons_ret_str) ::= A (N 0);;
+  invoke_subprogram cons_prefix cons_IMP_Minus;;
+
+  copy_var_to_operand_aux5_ret_str ::= A (V (cons_prefix @ cons_ret_str))
+"
+
+abbreviation "copy_var_to_operand_aux5_IMP_vars\<equiv>
+  {copy_var_to_operand_aux5_acc_str, copy_var_to_operand_aux5_diff_str,
+  copy_var_to_operand_aux5_i_str, copy_var_to_operand_aux5_op_str,
+  copy_var_to_operand_aux5_v_str, copy_var_to_operand_aux5_ret_str}"
+
+
+definition "copy_var_to_operand_aux5_imp_to_HOL_state p s =
+  \<lparr>copy_var_to_operand_aux5_acc = (s (add_prefix p copy_var_to_operand_aux5_acc_str)),
+  copy_var_to_operand_aux5_diff = (s (add_prefix p copy_var_to_operand_aux5_diff_str)),
+  copy_var_to_operand_aux5_i = (s (add_prefix p copy_var_to_operand_aux5_i_str)),
+  copy_var_to_operand_aux5_op = (s (add_prefix p copy_var_to_operand_aux5_op_str)),
+  copy_var_to_operand_aux5_v = (s (add_prefix p copy_var_to_operand_aux5_v_str)),
+  copy_var_to_operand_aux5_ret = (s (add_prefix p copy_var_to_operand_aux5_ret_str))\<rparr>"
+
+lemmas copy_var_to_operand_aux5_state_translators =
+  copy_var_to_operand_aux5_imp_to_HOL_state_def
+  cons_imp_to_HOL_state_def
+  copy_var_to_operand_aux4_imp_to_HOL_state_def
+
+lemma copy_var_to_operand_aux5_IMP_Minus_correct_function:
+  "(invoke_subprogram p copy_var_to_operand_aux5_IMP_Minus, s) \<Rightarrow>\<^bsup>t\<^esup> s' \<Longrightarrow>
+     s' (add_prefix p copy_var_to_operand_aux5_ret_str)
+      = copy_var_to_operand_aux5_ret
+          (copy_var_to_operand_aux5_imp (copy_var_to_operand_aux5_imp_to_HOL_state p s))"
+  apply (simp only: copy_var_to_operand_aux5_imp.simps copy_var_to_operand_aux5_state_upd_def)
+  apply (simp only: copy_var_to_operand_aux5_IMP_Minus_def prefix_simps)
+  apply (erule Seq_E)+
+  apply (erule cons_IMP_Minus_correct[where vars=copy_var_to_operand_aux5_IMP_vars])
+  subgoal premises p using p(19) by fastforce
+  apply (erule copy_var_to_operand_aux4_IMP_Minus_correct[where 
+         vars="copy_var_to_operand_aux5_IMP_vars \<union> {cons_prefix @ cons_ret_str}"])
+  subgoal premises p using p(21) by fastforce
+  apply (erule cons_IMP_Minus_correct[where vars=copy_var_to_operand_aux5_IMP_vars])
+  subgoal premises p using p(23) by fastforce
+  apply (erule cons_IMP_Minus_correct[where vars=copy_var_to_operand_aux5_IMP_vars])
+  subgoal premises p using p(25) by fastforce
+  apply (force simp: Let_def copy_var_to_operand_aux5_state_translators)
+  done 
+
+lemma copy_var_to_operand_aux5_IMP_Minus_correct_effects:
+  "\<lbrakk>(invoke_subprogram (p @ copy_var_to_operand_aux5_pref) copy_var_to_operand_aux5_IMP_Minus, s) \<Rightarrow>\<^bsup>t\<^esup> s';
+    v \<in> vars; \<not> (prefix copy_var_to_operand_aux5_pref v)\<rbrakk>
+   \<Longrightarrow> s (add_prefix p v) = s' (add_prefix p v)"
+  using com_add_prefix_valid'' com_only_vars prefix_def
+  by blast            
+
+lemma copy_var_to_operand_aux5_IMP_Minus_correct_time:
+  "(invoke_subprogram p copy_var_to_operand_aux5_IMP_Minus, s) \<Rightarrow>\<^bsup>t\<^esup> s' \<Longrightarrow>
+     t = copy_var_to_operand_aux5_imp_time 0 (copy_var_to_operand_aux5_imp_to_HOL_state p s)"
+  apply (simp only: copy_var_to_operand_aux5_imp_time.simps copy_var_to_operand_aux5_state_upd_time_def)
+  apply (simp only: copy_var_to_operand_aux5_IMP_Minus_def prefix_simps)
+  apply (erule Seq_tE)+
+  apply (erule cons_IMP_Minus_correct[where vars=copy_var_to_operand_aux5_IMP_vars])
+  subgoal premises p using p(37) by fastforce
+  apply (erule copy_var_to_operand_aux4_IMP_Minus_correct[where 
+         vars="copy_var_to_operand_aux5_IMP_vars \<union> {cons_prefix @ cons_ret_str}"])
+  subgoal premises p using p(39) by fastforce
+  apply (erule cons_IMP_Minus_correct[where vars=copy_var_to_operand_aux5_IMP_vars])
+  subgoal premises p using p(41) by fastforce
+  apply (erule cons_IMP_Minus_correct[where vars=copy_var_to_operand_aux5_IMP_vars])
+  subgoal premises p using p(43) by fastforce
+  apply (force simp: Let_def copy_var_to_operand_aux5_state_translators)
+  done 
+
+lemma copy_var_to_operand_aux5_IMP_Minus_correct:
+  "\<lbrakk>(invoke_subprogram (p1 @ p2) copy_var_to_operand_aux5_IMP_Minus, s) \<Rightarrow>\<^bsup>t\<^esup> s';
+    \<And>v. v \<in> vars \<Longrightarrow> \<not> (set p2 \<subseteq> set v);
+    \<lbrakk>t = (copy_var_to_operand_aux5_imp_time 0 (copy_var_to_operand_aux5_imp_to_HOL_state (p1 @ p2) s));
+     s' (add_prefix (p1 @ p2) copy_var_to_operand_aux5_ret_str) =
+          copy_var_to_operand_aux5_ret (copy_var_to_operand_aux5_imp
+                                        (copy_var_to_operand_aux5_imp_to_HOL_state (p1 @ p2) s));
+     \<And>v. v \<in> vars \<Longrightarrow> s (add_prefix p1 v) = s' (add_prefix p1 v)\<rbrakk>
+   \<Longrightarrow> P\<rbrakk> \<Longrightarrow> P"
+  using copy_var_to_operand_aux5_IMP_Minus_correct_function
+  by (auto simp: copy_var_to_operand_aux5_IMP_Minus_correct_time)
+    (meson copy_var_to_operand_aux5_IMP_Minus_correct_effects set_mono_prefix)
+
+subsubsection copy_var_to_operand_acc
+
+record copy_var_to_operand_acc_state =
+  copy_var_to_operand_acc_acc::nat
+  copy_var_to_operand_acc_diff::nat
+  copy_var_to_operand_acc_i::nat
+  copy_var_to_operand_acc_op::nat
+  copy_var_to_operand_acc_v::nat 
+  copy_var_to_operand_acc_ret::nat
+
+abbreviation "copy_var_to_operand_acc_prefix \<equiv> ''copy_var_to_operand_acc.''"
+abbreviation "copy_var_to_operand_acc_acc_str \<equiv> ''acc''"
+abbreviation "copy_var_to_operand_acc_diff_str \<equiv> ''diff''"
+abbreviation "copy_var_to_operand_acc_i_str \<equiv> ''i''"
+abbreviation "copy_var_to_operand_acc_op_str \<equiv> ''op''"
+abbreviation "copy_var_to_operand_acc_v_str \<equiv> ''v''"
+abbreviation "copy_var_to_operand_acc_ret_str \<equiv> ''ret''"
+
+definition "copy_var_to_operand_acc_state_upd s \<equiv>
+  (let 
+   copy_var_to_operand_aux5_acc' = copy_var_to_operand_acc_acc s;
+   copy_var_to_operand_aux5_diff' = copy_var_to_operand_acc_diff s;
+   copy_var_to_operand_aux5_i' = copy_var_to_operand_acc_i s;
+   copy_var_to_operand_aux5_op' = copy_var_to_operand_acc_op s;
+   copy_var_to_operand_aux5_v' = copy_var_to_operand_acc_v s;
+   copy_var_to_operand_aux5_ret' = 0;
+   copy_var_to_operand_aux5_state = 
+    \<lparr>copy_var_to_operand_aux5_acc = copy_var_to_operand_aux5_acc',
+    copy_var_to_operand_aux5_diff = copy_var_to_operand_aux5_diff',
+    copy_var_to_operand_aux5_i = copy_var_to_operand_aux5_i',
+    copy_var_to_operand_aux5_op = copy_var_to_operand_aux5_op',
+    copy_var_to_operand_aux5_v = copy_var_to_operand_aux5_v',
+    copy_var_to_operand_aux5_ret = copy_var_to_operand_aux5_ret'\<rparr>;
+  copy_var_to_operand_aux5_ret_state = copy_var_to_operand_aux5_imp copy_var_to_operand_aux5_state;
+
+  copy_var_to_operand_acc_acc' = copy_var_to_operand_aux5_ret copy_var_to_operand_aux5_ret_state;
+  copy_var_to_operand_acc_diff' = copy_var_to_operand_acc_diff s - 1;
+  ret = \<lparr>copy_var_to_operand_acc_acc = copy_var_to_operand_acc_acc',
+        copy_var_to_operand_acc_diff = copy_var_to_operand_acc_diff',
+        copy_var_to_operand_acc_i = copy_var_to_operand_acc_i s,
+        copy_var_to_operand_acc_op = copy_var_to_operand_acc_op s,
+        copy_var_to_operand_acc_v = copy_var_to_operand_acc_v s,
+        copy_var_to_operand_acc_ret = copy_var_to_operand_acc_ret s\<rparr>
+  in
+   ret)"
+
+
+definition "copy_var_to_operand_acc_imp_compute_loop_condition s \<equiv> 
+ (let
+  condition = copy_var_to_operand_acc_diff s
+ in 
+  condition)"
+
+definition "copy_var_to_operand_acc_imp_after_loop s \<equiv> 
+ (let 
+  copy_var_to_operand_acc_ret' = copy_var_to_operand_acc_acc s;
+  ret = \<lparr>copy_var_to_operand_acc_acc = copy_var_to_operand_acc_acc s,
+        copy_var_to_operand_acc_diff = copy_var_to_operand_acc_diff s,
+        copy_var_to_operand_acc_i = copy_var_to_operand_acc_i s,
+        copy_var_to_operand_acc_op = copy_var_to_operand_acc_op s,
+        copy_var_to_operand_acc_v = copy_var_to_operand_acc_v s,
+        copy_var_to_operand_acc_ret = copy_var_to_operand_acc_ret'\<rparr>
+ in
+  ret)"
+
+lemmas copy_var_to_operand_acc_imp_subprogram_simps = 
+  copy_var_to_operand_acc_state_upd_def
+  copy_var_to_operand_acc_imp_compute_loop_condition_def
+  copy_var_to_operand_acc_imp_after_loop_def
+
+function copy_var_to_operand_acc_imp::
+  "copy_var_to_operand_acc_state \<Rightarrow> copy_var_to_operand_acc_state" where
+  "copy_var_to_operand_acc_imp s =
+  (if copy_var_to_operand_acc_imp_compute_loop_condition s \<noteq> 0
+   then
+    let next_iteration = copy_var_to_operand_acc_imp (copy_var_to_operand_acc_state_upd s)
+    in next_iteration
+   else
+    let ret = copy_var_to_operand_acc_imp_after_loop s
+    in ret
+  )"
+  by simp+
+termination
+  apply (relation "measure copy_var_to_operand_acc_diff")
+  apply (simp add: copy_var_to_operand_acc_imp_subprogram_simps)+
+  done
+
+declare copy_var_to_operand_acc_imp.simps [simp del]
+
+lemma copy_var_to_operand_acc_imp_correct:
+  "copy_var_to_operand_acc_ret (copy_var_to_operand_acc_imp s) =
+    copy_var_to_operand_acc (copy_var_to_operand_acc_acc s) 
+    (copy_var_to_operand_acc_diff s) (copy_var_to_operand_acc_i s)
+    (copy_var_to_operand_acc_op s) (copy_var_to_operand_acc_v s)"
+  apply (induction s rule: copy_var_to_operand_acc_imp.induct)
+  apply (subst copy_var_to_operand_acc_imp.simps)
+  apply (subst copy_var_to_operand_acc.simps)
+  apply (auto simp del: copy_var_to_operand_acc.simps simp add: 
+  copy_var_to_operand_acc_imp_subprogram_simps Let_def
+  copy_var_to_operand_aux5_imp_correct)
+  done            
+
+
+definition "copy_var_to_operand_acc_state_upd_time t s \<equiv>
+  (let
+   copy_var_to_operand_aux5_acc' = copy_var_to_operand_acc_acc s;
+   t = t + 2;
+   copy_var_to_operand_aux5_diff' = copy_var_to_operand_acc_diff s;
+   t = t + 2;
+   copy_var_to_operand_aux5_i' = copy_var_to_operand_acc_i s;
+   t = t + 2;
+   copy_var_to_operand_aux5_op' = copy_var_to_operand_acc_op s;
+   t = t + 2;
+   copy_var_to_operand_aux5_v' = copy_var_to_operand_acc_v s;
+   t = t + 2;
+   copy_var_to_operand_aux5_ret' = 0;
+   t = t + 2;
+   copy_var_to_operand_aux5_state = 
+    \<lparr>copy_var_to_operand_aux5_acc = copy_var_to_operand_aux5_acc',
+    copy_var_to_operand_aux5_diff = copy_var_to_operand_aux5_diff',
+    copy_var_to_operand_aux5_i = copy_var_to_operand_aux5_i',
+    copy_var_to_operand_aux5_op = copy_var_to_operand_aux5_op',
+    copy_var_to_operand_aux5_v = copy_var_to_operand_aux5_v',
+    copy_var_to_operand_aux5_ret = copy_var_to_operand_aux5_ret'\<rparr>;
+  copy_var_to_operand_aux5_ret_state = copy_var_to_operand_aux5_imp copy_var_to_operand_aux5_state;
+   t = t + copy_var_to_operand_aux5_imp_time 0 copy_var_to_operand_aux5_state;
+
+  copy_var_to_operand_acc_acc' = copy_var_to_operand_aux5_ret copy_var_to_operand_aux5_ret_state;
+  t = t + 2;
+  copy_var_to_operand_acc_diff' = copy_var_to_operand_acc_diff s - 1;
+    t = t + 2;
+  ret = \<lparr>copy_var_to_operand_acc_acc = copy_var_to_operand_acc_acc',
+        copy_var_to_operand_acc_diff = copy_var_to_operand_acc_diff',
+        copy_var_to_operand_acc_i = copy_var_to_operand_acc_i s,
+        copy_var_to_operand_acc_op = copy_var_to_operand_acc_op s,
+        copy_var_to_operand_acc_v = copy_var_to_operand_acc_v s,
+        copy_var_to_operand_acc_ret = copy_var_to_operand_acc_ret s\<rparr>
+  in
+   t)"
+
+definition "copy_var_to_operand_acc_imp_compute_loop_condition_time t s \<equiv>
+  let
+  condition = copy_var_to_operand_acc_diff s;
+  t = t + 2
+  in
+    t
+"
+
+definition "copy_var_to_operand_acc_imp_after_loop_time t s \<equiv>
+  (let
+    copy_var_to_operand_acc_ret' = copy_var_to_operand_acc_acc s;
+    t = t + 2;
+    ret = \<lparr>copy_var_to_operand_acc_acc = copy_var_to_operand_acc_acc s,
+        copy_var_to_operand_acc_diff = copy_var_to_operand_acc_diff s,
+        copy_var_to_operand_acc_i = copy_var_to_operand_acc_i s,
+        copy_var_to_operand_acc_op = copy_var_to_operand_acc_op s,
+        copy_var_to_operand_acc_v = copy_var_to_operand_acc_v s,
+        copy_var_to_operand_acc_ret = copy_var_to_operand_acc_ret'\<rparr>
+  in
+    t)
+"
+
+lemmas copy_var_to_operand_acc_imp_subprogram_time_simps = 
+  copy_var_to_operand_acc_state_upd_time_def
+  copy_var_to_operand_acc_imp_compute_loop_condition_time_def
+  copy_var_to_operand_acc_imp_after_loop_time_def
+  copy_var_to_operand_acc_imp_subprogram_simps
+
+function copy_var_to_operand_acc_imp_time::
+  "nat \<Rightarrow> copy_var_to_operand_acc_state \<Rightarrow> nat" where
+  "copy_var_to_operand_acc_imp_time t s =
+  copy_var_to_operand_acc_imp_compute_loop_condition_time 0 s +
+  (if copy_var_to_operand_acc_imp_compute_loop_condition s \<noteq> 0
+    then
+      (let
+        t = t + 1;
+        next_iteration =
+          copy_var_to_operand_acc_imp_time (t + copy_var_to_operand_acc_state_upd_time 0 s)
+                         (copy_var_to_operand_acc_state_upd s)
+       in next_iteration)
+    else
+      (let
+        t = t + 2;
+        ret = t + copy_var_to_operand_acc_imp_after_loop_time 0 s
+       in ret)
+  )"
+  by auto
+termination
+  apply (relation "measure (copy_var_to_operand_acc_diff \<circ> snd)")
+  by (simp add: copy_var_to_operand_acc_imp_subprogram_time_simps)+
+
+declare copy_var_to_operand_acc_imp_time.simps [simp del]            
+
+lemma copy_var_to_operand_acc_imp_time_acc:
+  "(copy_var_to_operand_acc_imp_time (Suc t) s) = Suc (copy_var_to_operand_acc_imp_time t s)"
+  by (induction t s rule: copy_var_to_operand_acc_imp_time.induct)
+    ((subst (1 2) copy_var_to_operand_acc_imp_time.simps);
+      (simp add: copy_var_to_operand_acc_state_upd_def))            
+
+lemma copy_var_to_operand_acc_imp_time_acc_2_aux:
+  "(copy_var_to_operand_acc_imp_time t s) = t + (copy_var_to_operand_acc_imp_time 0 s)"
+  by (induction t arbitrary: s) (simp add: copy_var_to_operand_acc_imp_time_acc)+            
+
+lemma copy_var_to_operand_acc_imp_time_acc_2:
+  "t \<noteq> 0 \<Longrightarrow> (copy_var_to_operand_acc_imp_time t s) = t + (copy_var_to_operand_acc_imp_time 0 s)"
+  by (rule copy_var_to_operand_acc_imp_time_acc_2_aux)            
+
+lemma copy_var_to_operand_acc_imp_time_acc_3:
+  "(copy_var_to_operand_acc_imp_time (a + b) s) = a + (copy_var_to_operand_acc_imp_time b s)"
+  by (induction a arbitrary: b s) (simp add: copy_var_to_operand_acc_imp_time_acc)+            
+
+abbreviation "copy_var_to_operand_acc_while_cond \<equiv> ''condition''"
+
+definition "copy_var_to_operand_acc_IMP_init_while_cond \<equiv>
+  copy_var_to_operand_acc_while_cond ::= A (V copy_var_to_operand_acc_diff_str)
+"
+
+definition "copy_var_to_operand_acc_IMP_loop_body \<equiv>
+  (copy_var_to_operand_aux5_prefix @ copy_var_to_operand_aux5_acc_str) 
+    ::= A (V (copy_var_to_operand_acc_acc_str));;
+  (copy_var_to_operand_aux5_prefix @ copy_var_to_operand_aux5_diff_str) 
+    ::= A (V (copy_var_to_operand_acc_diff_str));;
+  (copy_var_to_operand_aux5_prefix @ copy_var_to_operand_aux5_i_str) 
+    ::= A (V copy_var_to_operand_acc_i_str);;
+  (copy_var_to_operand_aux5_prefix @ copy_var_to_operand_aux5_op_str) 
+    ::= A (V copy_var_to_operand_acc_op_str);;
+  (copy_var_to_operand_aux5_prefix @ copy_var_to_operand_aux5_v_str) 
+    ::= A (V copy_var_to_operand_acc_v_str);;
+  (copy_var_to_operand_aux5_prefix @ copy_var_to_operand_aux5_ret_str) 
+    ::= A (N 0);;
+  invoke_subprogram copy_var_to_operand_aux5_prefix copy_var_to_operand_aux5_IMP_Minus;;
+
+  copy_var_to_operand_acc_acc_str ::= A (V (copy_var_to_operand_aux5_prefix @ copy_var_to_operand_aux5_ret_str) );;
+  copy_var_to_operand_acc_diff_str ::= Sub (V copy_var_to_operand_acc_diff_str) (N 1)
+"
+
+definition "copy_var_to_operand_acc_IMP_after_loop \<equiv>
+  copy_var_to_operand_acc_ret_str ::= A (V copy_var_to_operand_acc_acc_str)
+"
+
+definition copy_var_to_operand_acc_IMP_Minus where
+  "copy_var_to_operand_acc_IMP_Minus \<equiv>
+  copy_var_to_operand_acc_IMP_init_while_cond;;
+  WHILE copy_var_to_operand_acc_while_cond \<noteq>0 DO (
+    copy_var_to_operand_acc_IMP_loop_body;;
+    copy_var_to_operand_acc_IMP_init_while_cond
+  );;
+  copy_var_to_operand_acc_IMP_after_loop"
+
+abbreviation "copy_var_to_operand_acc_IMP_vars\<equiv>
+  {copy_var_to_operand_acc_acc_str, copy_var_to_operand_acc_diff_str,
+  copy_var_to_operand_acc_i_str, copy_var_to_operand_acc_op_str,
+  copy_var_to_operand_acc_v_str, copy_var_to_operand_acc_ret_str,
+  copy_var_to_operand_acc_while_cond}"
+
+lemmas copy_var_to_operand_acc_IMP_subprogram_simps =
+  copy_var_to_operand_acc_IMP_init_while_cond_def
+  copy_var_to_operand_acc_IMP_loop_body_def
+  copy_var_to_operand_acc_IMP_after_loop_def
+
+definition "copy_var_to_operand_acc_imp_to_HOL_state p s =
+  \<lparr>copy_var_to_operand_acc_acc = (s (add_prefix p copy_var_to_operand_acc_acc_str)),
+  copy_var_to_operand_acc_diff = (s (add_prefix p copy_var_to_operand_acc_diff_str)),
+  copy_var_to_operand_acc_i = (s (add_prefix p copy_var_to_operand_acc_i_str)),
+  copy_var_to_operand_acc_op = (s (add_prefix p copy_var_to_operand_acc_op_str)),
+  copy_var_to_operand_acc_v = (s (add_prefix p copy_var_to_operand_acc_v_str)),
+  copy_var_to_operand_acc_ret = (s (add_prefix p copy_var_to_operand_acc_ret_str))\<rparr>"
+
+lemmas copy_var_to_operand_acc_state_translators =
+  copy_var_to_operand_acc_imp_to_HOL_state_def
+  cons_imp_to_HOL_state_def
+  copy_var_to_operand_aux5_imp_to_HOL_state_def
+
+lemmas copy_var_to_operand_acc_complete_simps =
+  copy_var_to_operand_acc_IMP_subprogram_simps
+  copy_var_to_operand_acc_imp_subprogram_simps
+  copy_var_to_operand_acc_state_translators
+
+lemma copy_var_to_operand_acc_IMP_Minus_correct_function:
+  "(invoke_subprogram p copy_var_to_operand_acc_IMP_Minus, s) \<Rightarrow>\<^bsup>t\<^esup> s' \<Longrightarrow>
+     s' (add_prefix p copy_var_to_operand_acc_ret_str)
+      = copy_var_to_operand_acc_ret
+          (copy_var_to_operand_acc_imp (copy_var_to_operand_acc_imp_to_HOL_state p s))"
+  apply(induction "copy_var_to_operand_acc_imp_to_HOL_state p s" arbitrary: s s' t
+    rule: copy_var_to_operand_acc_imp.induct)
+  apply(subst copy_var_to_operand_acc_imp.simps)
+  apply(simp only: copy_var_to_operand_acc_IMP_Minus_def prefix_simps)
+  apply(erule Seq_E)+
+  apply(erule While_tE)
+
+  subgoal
+    apply(simp only: copy_var_to_operand_acc_IMP_subprogram_simps prefix_simps)
+    by(fastforce simp: copy_var_to_operand_acc_IMP_subprogram_simps
+        copy_var_to_operand_acc_imp_subprogram_simps
+        copy_var_to_operand_acc_state_translators)
+
+  apply(erule Seq_E)+
+  apply(dest_com_gen)
+
+  subgoal
+      apply(simp only: copy_var_to_operand_acc_IMP_init_while_cond_def prefix_simps)
+      by(fastforce simp add: copy_var_to_operand_acc_complete_simps)
+
+  subgoal
+      apply(subst (asm) copy_var_to_operand_acc_IMP_init_while_cond_def)
+      apply(simp only: copy_var_to_operand_acc_IMP_loop_body_def prefix_simps)
+      apply(erule Seq_E)+
+      apply(erule copy_var_to_operand_aux5_IMP_Minus_correct[where vars = copy_var_to_operand_acc_IMP_vars])
+      subgoal premises p using p(14) by fastforce
+      by (force simp: copy_var_to_operand_acc_imp_subprogram_simps
+          copy_var_to_operand_acc_state_translators Let_def)
+
+  subgoal
+      apply(simp only: copy_var_to_operand_acc_IMP_init_while_cond_def prefix_simps
+          copy_var_to_operand_acc_IMP_loop_body_def)
+      apply(erule Seq_E)+
+      apply(erule copy_var_to_operand_aux5_IMP_Minus_correct[where vars = copy_var_to_operand_acc_IMP_vars])
+      subgoal premises p using p(14) by fastforce
+      by (force simp: copy_var_to_operand_acc_imp_subprogram_simps
+          copy_var_to_operand_acc_state_translators Let_def)
+  done        
+
+lemma copy_var_to_operand_acc_IMP_Minus_correct_effects:
+  "\<lbrakk>(invoke_subprogram (p @ copy_var_to_operand_acc_pref) copy_var_to_operand_acc_IMP_Minus, s) \<Rightarrow>\<^bsup>t\<^esup> s';
+    v \<in> vars; \<not> (prefix copy_var_to_operand_acc_pref v)\<rbrakk>
+   \<Longrightarrow> s (add_prefix p v) = s' (add_prefix p v)"
+  using com_add_prefix_valid'' com_only_vars prefix_def
+  by blast            
+
+lemmas copy_var_to_operand_acc_complete_time_simps =
+  copy_var_to_operand_acc_imp_subprogram_time_simps
+  copy_var_to_operand_acc_imp_time_acc_2
+  copy_var_to_operand_acc_imp_time_acc_3
+  copy_var_to_operand_acc_state_translators
+
+lemma copy_var_to_operand_acc_IMP_Minus_correct_time:
+  "(invoke_subprogram p copy_var_to_operand_acc_IMP_Minus, s) \<Rightarrow>\<^bsup>t\<^esup> s' \<Longrightarrow>
+     t = copy_var_to_operand_acc_imp_time 0 (copy_var_to_operand_acc_imp_to_HOL_state p s)"
+  apply(induction "copy_var_to_operand_acc_imp_to_HOL_state p s" arbitrary: s s' t
+      rule: copy_var_to_operand_acc_imp.induct)
+  apply(subst copy_var_to_operand_acc_imp_time.simps)
+  apply(simp only: copy_var_to_operand_acc_IMP_Minus_def prefix_simps)
+
+  apply(erule Seq_tE)+
+  apply(erule While_tE_time)
+
+  subgoal
+    apply(simp only: copy_var_to_operand_acc_IMP_subprogram_simps prefix_simps)
+    by (force simp: copy_var_to_operand_acc_IMP_subprogram_simps
+        copy_var_to_operand_acc_imp_subprogram_time_simps copy_var_to_operand_acc_state_translators)
+
+  apply(erule Seq_tE)+
+  apply(simp add: add.assoc)
+  apply(dest_com_gen_time)
+
+  subgoal
+    apply(simp only: copy_var_to_operand_acc_IMP_init_while_cond_def prefix_simps)
+    by(fastforce simp add: copy_var_to_operand_acc_complete_simps)
+
+  subgoal
+    apply(subst (asm) copy_var_to_operand_acc_IMP_init_while_cond_def)
+    apply(simp only: copy_var_to_operand_acc_IMP_loop_body_def prefix_simps)
+    apply(erule Seq_tE)+
+    apply(erule copy_var_to_operand_aux5_IMP_Minus_correct[where vars = copy_var_to_operand_acc_IMP_vars])
+    subgoal premises p using p(25) by fastforce
+    by (force simp: copy_var_to_operand_acc_imp_subprogram_simps
+          copy_var_to_operand_acc_state_translators Let_def)
+
+  subgoal
+    apply(simp only: prefix_simps copy_var_to_operand_acc_IMP_init_while_cond_def
+        copy_var_to_operand_acc_IMP_loop_body_def)
+    apply(erule Seq_tE)+
+    apply(erule copy_var_to_operand_aux5_IMP_Minus_correct[where vars = copy_var_to_operand_acc_IMP_vars])
+    subgoal premises p using p(25) by fastforce
+    apply (force simp: copy_var_to_operand_acc_complete_time_simps Let_def)
+    done      
+  done        
+
+lemma copy_var_to_operand_acc_IMP_Minus_correct:
+  "\<lbrakk>(invoke_subprogram (p1 @ p2) copy_var_to_operand_acc_IMP_Minus, s) \<Rightarrow>\<^bsup>t\<^esup> s';
+    \<And>v. v \<in> vars \<Longrightarrow> \<not> (set p2 \<subseteq> set v);
+    \<lbrakk>t = (copy_var_to_operand_acc_imp_time 0 (copy_var_to_operand_acc_imp_to_HOL_state (p1 @ p2) s));
+     s' (add_prefix (p1 @ p2) copy_var_to_operand_acc_ret_str) =
+          copy_var_to_operand_acc_ret (copy_var_to_operand_acc_imp
+                                        (copy_var_to_operand_acc_imp_to_HOL_state (p1 @ p2) s));
+     \<And>v. v \<in> vars \<Longrightarrow> s (add_prefix p1 v) = s' (add_prefix p1 v)\<rbrakk>
+   \<Longrightarrow> P\<rbrakk> \<Longrightarrow> P"
+  using copy_var_to_operand_acc_IMP_Minus_correct_function
+  by (auto simp: copy_var_to_operand_acc_IMP_Minus_correct_time)
+    (meson copy_var_to_operand_acc_IMP_Minus_correct_effects set_mono_prefix) 
+
+subsubsection copy_var_to_operand_tail 
+
+record copy_var_to_operand_tail_state =
+  copy_var_to_operand_tail_i::nat
+  copy_var_to_operand_tail_op::nat 
+  copy_var_to_operand_tail_v::nat
+  copy_var_to_operand_tail_ret::nat
+
+abbreviation "copy_var_to_operand_tail_prefix \<equiv> ''copy_var_to_operand_tail.''"
+abbreviation "copy_var_to_operand_tail_i_str \<equiv> ''i''"
+abbreviation "copy_var_to_operand_tail_op_str \<equiv> ''op''"
+abbreviation "copy_var_to_operand_tail_v_str \<equiv> ''v''"
+abbreviation "copy_var_to_operand_tail_ret_str \<equiv> ''ret''"
+
+definition "copy_var_to_operand_tail_state_upd s \<equiv> 
+(let
+  cons_h' = 0;
+  cons_t' = 0;
+  cons_ret' = 0;
+  cons_state = \<lparr>cons_h = cons_h', cons_t = cons_t', cons_ret = cons_ret'\<rparr>;
+  cons_ret_state = cons_imp cons_state;
+
+  copy_var_to_operand_acc_acc' = cons_ret cons_ret_state;
+  copy_var_to_operand_acc_diff' = copy_var_to_operand_tail_i s;
+  copy_var_to_operand_acc_i' = copy_var_to_operand_tail_i s;
+  copy_var_to_operand_acc_op' = copy_var_to_operand_tail_op s;
+  copy_var_to_operand_acc_v' = copy_var_to_operand_tail_v s;
+  copy_var_to_operand_acc_ret' = 0;
+  copy_var_to_operand_acc_state = 
+    \<lparr>copy_var_to_operand_acc_acc = copy_var_to_operand_acc_acc',
+    copy_var_to_operand_acc_diff = copy_var_to_operand_acc_diff',
+    copy_var_to_operand_acc_i = copy_var_to_operand_acc_i',
+    copy_var_to_operand_acc_op = copy_var_to_operand_acc_op',
+    copy_var_to_operand_acc_v = copy_var_to_operand_acc_v',
+    copy_var_to_operand_acc_ret = copy_var_to_operand_acc_ret'\<rparr>;
+  copy_var_to_operand_acc_ret_state = copy_var_to_operand_acc_imp copy_var_to_operand_acc_state;
+
+  copy_var_to_operand_tail_ret' = copy_var_to_operand_acc_ret copy_var_to_operand_acc_ret_state;
+  ret = 
+    \<lparr>copy_var_to_operand_tail_i = copy_var_to_operand_tail_i s,
+    copy_var_to_operand_tail_op = copy_var_to_operand_tail_op s,
+    copy_var_to_operand_tail_v = copy_var_to_operand_tail_v s,
+    copy_var_to_operand_tail_ret = copy_var_to_operand_tail_ret'\<rparr>
+  in 
+   ret)"
+
+function copy_var_to_operand_tail_imp 
+ :: "copy_var_to_operand_tail_state \<Rightarrow> copy_var_to_operand_tail_state" where 
+"copy_var_to_operand_tail_imp s = 
+ (let
+   ret = copy_var_to_operand_tail_state_upd s
+  in
+   ret)" by simp+
+  termination by (relation "measure copy_var_to_operand_tail_i", simp)
+
+declare copy_var_to_operand_tail_imp.simps[simp del]
+
+lemma copy_var_to_operand_tail_imp_correct:
+  "copy_var_to_operand_tail_ret (copy_var_to_operand_tail_imp s) =
+    copy_var_to_operand_tail (copy_var_to_operand_tail_i s) 
+     (copy_var_to_operand_tail_op s) (copy_var_to_operand_tail_v s)"
+apply (simp only: copy_var_to_operand_tail_imp.simps copy_var_to_operand_tail_state_upd_def)
+apply (simp add: copy_var_to_operand_acc_imp_correct cons_imp_correct 
+      Let_def copy_var_to_operand_tail_def)
+done 
+
+definition "copy_var_to_operand_tail_state_upd_time t s \<equiv> 
+(let
+  cons_h' = 0;
+  t = t + 2;
+  cons_t' = 0;
+  t = t + 2;
+  cons_ret' = 0;
+  t = t + 2;
+  cons_state = \<lparr>cons_h = cons_h', cons_t = cons_t', cons_ret = cons_ret'\<rparr>;
+  cons_ret_state = cons_imp cons_state;
+  t = t + cons_imp_time 0 cons_state;
+
+  copy_var_to_operand_acc_acc' = cons_ret cons_ret_state;
+  t = t + 2;
+  t = t + 2;
+  copy_var_to_operand_acc_diff' = copy_var_to_operand_tail_i s;
+  copy_var_to_operand_acc_i' = copy_var_to_operand_tail_i s;
+  t = t + 2;
+  copy_var_to_operand_acc_op' = copy_var_to_operand_tail_op s;
+  t = t + 2;
+  copy_var_to_operand_acc_v' = copy_var_to_operand_tail_v s;
+  t = t + 2;
+  copy_var_to_operand_acc_ret' = 0;
+  t = t + 2;
+  copy_var_to_operand_acc_state = 
+    \<lparr>copy_var_to_operand_acc_acc = copy_var_to_operand_acc_acc',
+    copy_var_to_operand_acc_diff = copy_var_to_operand_acc_diff',
+    copy_var_to_operand_acc_i = copy_var_to_operand_acc_i',
+    copy_var_to_operand_acc_op = copy_var_to_operand_acc_op',
+    copy_var_to_operand_acc_v = copy_var_to_operand_acc_v',
+    copy_var_to_operand_acc_ret = copy_var_to_operand_acc_ret'\<rparr>;
+  copy_var_to_operand_acc_ret_state = copy_var_to_operand_acc_imp copy_var_to_operand_acc_state;
+  t = t + copy_var_to_operand_acc_imp_time 0 copy_var_to_operand_acc_state;
+
+  copy_var_to_operand_tail_ret' = copy_var_to_operand_acc_ret copy_var_to_operand_acc_ret_state;
+  t = t + 2;
+  ret = 
+    \<lparr>copy_var_to_operand_tail_i = copy_var_to_operand_tail_i s,
+    copy_var_to_operand_tail_op = copy_var_to_operand_tail_op s,
+    copy_var_to_operand_tail_v = copy_var_to_operand_tail_v s,
+    copy_var_to_operand_tail_ret = copy_var_to_operand_tail_ret'\<rparr>
+  in 
+   t)"
+
+function copy_var_to_operand_tail_imp_time 
+ :: "nat \<Rightarrow> copy_var_to_operand_tail_state \<Rightarrow> nat" where 
+"copy_var_to_operand_tail_imp_time t s = 
+ (let
+   ret = copy_var_to_operand_tail_state_upd s;
+   t = t + copy_var_to_operand_tail_state_upd_time 0 s
+  in
+   t)" by auto
+  termination by (relation "measure (copy_var_to_operand_tail_i \<circ> snd)", simp)
+
+declare copy_var_to_operand_tail_imp_time.simps[simp del]
+
+abbreviation "copy_var_to_operand_tail_IMP_vars \<equiv> 
+  {copy_var_to_operand_tail_i_str, copy_var_to_operand_tail_op_str, 
+  copy_var_to_operand_tail_v_str, copy_var_to_operand_tail_ret_str}"
+
+definition "copy_var_to_operand_tail_imp_to_HOL_state p s \<equiv>
+  \<lparr>copy_var_to_operand_tail_i = s (add_prefix p copy_var_to_operand_tail_i_str),
+  copy_var_to_operand_tail_op = s (add_prefix p copy_var_to_operand_tail_op_str),
+  copy_var_to_operand_tail_v = s (add_prefix p copy_var_to_operand_tail_v_str),
+  copy_var_to_operand_tail_ret = s (add_prefix p copy_var_to_operand_tail_ret_str)\<rparr>"
+
+definition "copy_var_to_operand_tail_IMP_Minus \<equiv> 
+  (cons_prefix @ cons_h_str) ::= A (N 0);;
+  (cons_prefix @ cons_t_str) ::= A (N 0);;
+  (cons_prefix @ cons_ret_str) ::= A (N 0);;
+  invoke_subprogram cons_prefix cons_IMP_Minus;;
+  
+  (copy_var_to_operand_acc_prefix @ copy_var_to_operand_acc_acc_str)
+    ::= A (V (cons_prefix @ cons_ret_str));;
+  (copy_var_to_operand_acc_prefix @ copy_var_to_operand_acc_diff_str)
+    ::= A (V copy_var_to_operand_tail_i_str);;
+  (copy_var_to_operand_acc_prefix @ copy_var_to_operand_acc_i_str)
+    ::= A (V copy_var_to_operand_tail_i_str);;
+  (copy_var_to_operand_acc_prefix @ copy_var_to_operand_acc_op_str)
+    ::= A (V copy_var_to_operand_tail_op_str);;
+  (copy_var_to_operand_acc_prefix @ copy_var_to_operand_acc_v_str)
+    ::= A (V copy_var_to_operand_tail_v_str);;
+  (copy_var_to_operand_acc_prefix @ copy_var_to_operand_acc_ret_str)
+    ::= A (N 0);;
+  invoke_subprogram  copy_var_to_operand_acc_prefix  copy_var_to_operand_acc_IMP_Minus;;
+  
+  copy_var_to_operand_tail_ret_str 
+    ::= A (V (copy_var_to_operand_acc_prefix @ copy_var_to_operand_acc_ret_str))
+    
+  "
+
+lemmas copy_var_to_operand_tail_state_translators=
+  copy_var_to_operand_tail_imp_to_HOL_state_def
+  copy_var_to_operand_acc_imp_to_HOL_state_def
+  cons_imp_to_HOL_state_def
+
+lemma copy_var_to_operand_tail_IMP_Minus_correct_function:
+  "(invoke_subprogram p copy_var_to_operand_tail_IMP_Minus, s) \<Rightarrow>\<^bsup>t\<^esup> s' \<Longrightarrow>
+     s' (add_prefix p copy_var_to_operand_tail_ret_str)
+      = copy_var_to_operand_tail_ret
+          (copy_var_to_operand_tail_imp (copy_var_to_operand_tail_imp_to_HOL_state p s))"
+apply (simp only: copy_var_to_operand_tail_imp.simps copy_var_to_operand_tail_state_upd_def)
+apply (simp only: copy_var_to_operand_tail_IMP_Minus_def prefix_simps)
+apply (erule Seq_E)+
+apply (erule cons_IMP_Minus_correct[where vars=copy_var_to_operand_tail_IMP_vars])
+subgoal premises p using p(12) by fastforce
+apply (erule copy_var_to_operand_acc_IMP_Minus_correct[where vars=copy_var_to_operand_tail_IMP_vars])
+subgoal premises p using p(14) by fastforce
+apply (force simp add: copy_var_to_operand_tail_state_translators Let_def)
+done 
+
+lemma copy_var_to_operand_tail_IMP_Minus_correct_time:
+  "(invoke_subprogram p copy_var_to_operand_tail_IMP_Minus, s) \<Rightarrow>\<^bsup>t\<^esup> s' \<Longrightarrow>
+     t = (copy_var_to_operand_tail_imp_time 0 (copy_var_to_operand_tail_imp_to_HOL_state p s))"
+apply (simp only: copy_var_to_operand_tail_imp_time.simps copy_var_to_operand_tail_state_upd_time_def)
+apply (simp only: copy_var_to_operand_tail_IMP_Minus_def prefix_simps)
+apply (erule Seq_tE)+
+apply (erule cons_IMP_Minus_correct[where vars=copy_var_to_operand_tail_IMP_vars])
+subgoal premises p using p(23) by fastforce
+apply (erule copy_var_to_operand_acc_IMP_Minus_correct[where vars=copy_var_to_operand_tail_IMP_vars])
+subgoal premises p using p(25) by fastforce
+apply (force simp add: copy_var_to_operand_tail_state_translators Let_def)
+done 
+
+lemma copy_var_to_operand_tail_IMP_Minus_correct_effects:
+  "\<lbrakk>(invoke_subprogram (p @ copy_var_to_operand_tail_pref) copy_var_to_operand_tail_IMP_Minus, s) \<Rightarrow>\<^bsup>t\<^esup> s';
+    v \<in> vars; \<not> (prefix copy_var_to_operand_tail_pref v)\<rbrakk>
+   \<Longrightarrow> s (add_prefix p v) = s' (add_prefix p v)"
+  using com_add_prefix_valid'' com_only_vars prefix_def
+  by blast
+
+lemma copy_var_to_operand_tail_IMP_Minus_correct:
+  "\<lbrakk>(invoke_subprogram (p1 @ p2) copy_var_to_operand_tail_IMP_Minus, s) \<Rightarrow>\<^bsup>t\<^esup> s';
+    \<And>v. v \<in> vars \<Longrightarrow> \<not> (set p2 \<subseteq> set v);
+    \<lbrakk>t = (copy_var_to_operand_tail_imp_time 0 (copy_var_to_operand_tail_imp_to_HOL_state (p1 @ p2) s));
+     s' (add_prefix (p1 @ p2) copy_var_to_operand_tail_ret_str) =
+          copy_var_to_operand_tail_ret (copy_var_to_operand_tail_imp
+                                        (copy_var_to_operand_tail_imp_to_HOL_state (p1 @ p2) s));
+     \<And>v. v \<in> vars \<Longrightarrow> s (add_prefix p1 v) = s' (add_prefix p1 v)\<rbrakk>
+   \<Longrightarrow> P\<rbrakk> \<Longrightarrow> P"
+  using copy_var_to_operand_tail_IMP_Minus_correct_function
+  by (auto simp: copy_var_to_operand_tail_IMP_Minus_correct_time)
+    (meson copy_var_to_operand_tail_IMP_Minus_correct_effects set_mono_prefix) 
+
+subsection copy_const_to_operand
+
+subsubsection copy_const_to_operand_aux1
+
+record copy_const_to_operand_aux1_state =
+  copy_const_to_operand_aux1_x::nat
+  copy_const_to_operand_aux1_diff::nat
+  copy_const_to_operand_aux1_op::nat
+  copy_const_to_operand_aux1_ret::nat
+
+abbreviation "copy_const_to_operand_aux1_prefix \<equiv> ''copy_const_to_operand_aux1.''"
+abbreviation "copy_const_to_operand_aux1_x_str \<equiv> ''x''"
+abbreviation "copy_const_to_operand_aux1_diff_str \<equiv> ''diff''"
+abbreviation "copy_const_to_operand_aux1_op_str \<equiv> ''op''"
+abbreviation "copy_const_to_operand_aux1_ret_str \<equiv> ''ret''"
+
+definition "copy_const_to_operand_aux1_imp s \<equiv> 
+(let
+  nth_bit_tail_acc' = copy_const_to_operand_aux1_x s;
+  nth_bit_tail_n' = copy_const_to_operand_aux1_diff s;
+  nth_bit_tail_ret' = 0;
+  nth_bit_tail_state = \<lparr>nth_bit_tail_acc = nth_bit_tail_acc',
+                        nth_bit_tail_n = nth_bit_tail_n',
+                        nth_bit_tail_ret = nth_bit_tail_ret'\<rparr>;
+  nth_bit_tail_ret_state = nth_bit_tail_imp nth_bit_tail_state;
+
+  cons_h' = nth_bit_tail_ret nth_bit_tail_ret_state;
+  cons_t' = 0;
+  cons_ret' = 0;
+  cons_state = \<lparr>cons_h = cons_h', cons_t = cons_t', cons_ret = cons_ret'\<rparr>;
+  cons_ret_state = cons_imp cons_state;
+
+  prod_encode_a' = copy_const_to_operand_aux1_op s;
+  prod_encode_b' = copy_const_to_operand_aux1_diff s;
+  prod_encode_ret' = 0;
+  prod_encode_state = \<lparr>prod_encode_a = prod_encode_a', 
+                       prod_encode_b = prod_encode_b',
+                       prod_encode_ret = prod_encode_ret'\<rparr>;
+  prod_encode_ret_state = prod_encode_imp prod_encode_state;
+
+  operand_bit_to_var_tail_n' = prod_encode_ret prod_encode_ret_state;
+  operand_bit_to_var_tail_ret' = 0;
+  operand_bit_to_var_tail_state = 
+    \<lparr>operand_bit_to_var_tail_n = operand_bit_to_var_tail_n',
+    operand_bit_to_var_tail_ret = operand_bit_to_var_tail_ret'\<rparr>;
+  operand_bit_to_var_tail_ret_state 
+    = operand_bit_to_var_tail_imp operand_bit_to_var_tail_state;
+
+  cons_h' = operand_bit_to_var_tail_ret operand_bit_to_var_tail_ret_state;
+  cons_t' = cons_ret cons_ret_state;
+  cons_ret' = 0;
+  cons_state = \<lparr>cons_h = cons_h', cons_t = cons_t', cons_ret = cons_ret'\<rparr>;
+  cons_ret_state = cons_imp  cons_state;
+
+  cons_h' = 1;
+  cons_t' = cons_ret cons_ret_state;
+  cons_ret' = 0;
+  cons_state = \<lparr>cons_h = cons_h', cons_t = cons_t', cons_ret = cons_ret'\<rparr>;
+  cons_ret_state = cons_imp  cons_state;
+
+  copy_const_to_operand_aux1_ret' = cons_ret cons_ret_state;
+  ret = \<lparr>copy_const_to_operand_aux1_x = copy_const_to_operand_aux1_x s,
+        copy_const_to_operand_aux1_diff = copy_const_to_operand_aux1_diff s,
+        copy_const_to_operand_aux1_op = copy_const_to_operand_aux1_op s,
+        copy_const_to_operand_aux1_ret = copy_const_to_operand_aux1_ret'\<rparr>
+in
+ ret)"
+
+lemma copy_const_to_operand_aux1_imp_correct:
+  "copy_const_to_operand_aux1_ret (copy_const_to_operand_aux1_imp s) 
+  = (1 ## (operand_bit_to_var_tail (prod_encode 
+    (copy_const_to_operand_aux1_op s,copy_const_to_operand_aux1_diff s))) 
+## (nth_bit_tail (copy_const_to_operand_aux1_x s) (copy_const_to_operand_aux1_diff s)) 
+## 0)"
+apply (simp only: copy_const_to_operand_aux1_imp_def)
+apply (simp add: Let_def cons_imp_correct nth_bit_tail_imp_correct
+   operand_bit_to_var_tail_imp_correct prod_encode_imp_correct nth_bit_tail'_correct)
+done 
+
+definition "copy_const_to_operand_aux1_imp_time t s \<equiv> 
+(let
+  nth_bit_tail_acc' = copy_const_to_operand_aux1_x s;
+  t = t + 2;
+  nth_bit_tail_n' = copy_const_to_operand_aux1_diff s;
+  t = t + 2;
+  nth_bit_tail_ret' = 0;
+  t = t + 2;
+  nth_bit_tail_state = \<lparr>nth_bit_tail_acc = nth_bit_tail_acc',
+                        nth_bit_tail_n = nth_bit_tail_n',
+                        nth_bit_tail_ret = nth_bit_tail_ret'\<rparr>;
+  nth_bit_tail_ret_state = nth_bit_tail_imp nth_bit_tail_state;
+  t = t + nth_bit_tail_imp_time 0 nth_bit_tail_state;
+
+  cons_h' = nth_bit_tail_ret nth_bit_tail_ret_state;
+  t = t + 2;
+  cons_t' = 0;
+  t = t + 2;
+  cons_ret' = 0;
+  t = t + 2;
+  cons_state = \<lparr>cons_h = cons_h', cons_t = cons_t', cons_ret = cons_ret'\<rparr>;
+  cons_ret_state = cons_imp cons_state;
+  t = t + cons_imp_time 0 cons_state;
+
+  prod_encode_a' = copy_const_to_operand_aux1_op s;
+  t = t + 2;
+  prod_encode_b' = copy_const_to_operand_aux1_diff s;
+  t = t + 2;
+  prod_encode_ret' = 0;
+  t = t + 2;
+  prod_encode_state = \<lparr>prod_encode_a = prod_encode_a', 
+                       prod_encode_b = prod_encode_b',
+                       prod_encode_ret = prod_encode_ret'\<rparr>;
+  prod_encode_ret_state = prod_encode_imp prod_encode_state;
+  t = t + prod_encode_imp_time 0 prod_encode_state;
+
+  operand_bit_to_var_tail_n' = prod_encode_ret prod_encode_ret_state;
+  t = t + 2;
+  operand_bit_to_var_tail_ret' = 0;
+  t = t + 2;
+  operand_bit_to_var_tail_state = 
+    \<lparr>operand_bit_to_var_tail_n = operand_bit_to_var_tail_n',
+    operand_bit_to_var_tail_ret = operand_bit_to_var_tail_ret'\<rparr>;
+  operand_bit_to_var_tail_ret_state 
+    = operand_bit_to_var_tail_imp operand_bit_to_var_tail_state;
+  t = t + operand_bit_to_var_tail_imp_time 0 operand_bit_to_var_tail_state;
+
+  cons_h' = operand_bit_to_var_tail_ret operand_bit_to_var_tail_ret_state;
+  t = t + 2;
+  cons_t' = cons_ret cons_ret_state;
+  t = t + 2;
+  cons_ret' = 0;
+  t = t + 2;
+  cons_state = \<lparr>cons_h = cons_h', cons_t = cons_t', cons_ret = cons_ret'\<rparr>;
+  cons_ret_state = cons_imp  cons_state;
+  t = t + cons_imp_time 0 cons_state;
+
+  cons_h' = 1;
+  t = t + 2;
+  cons_t' = cons_ret cons_ret_state;
+  t = t + 2;
+  cons_ret' = 0;
+  t = t + 2;
+  cons_state = \<lparr>cons_h = cons_h', cons_t = cons_t', cons_ret = cons_ret'\<rparr>;
+  cons_ret_state = cons_imp  cons_state;
+  t = t + cons_imp_time 0 cons_state;
+
+  copy_const_to_operand_aux1_ret' = cons_ret cons_ret_state;
+  t = t + 2;
+  ret = \<lparr>copy_const_to_operand_aux1_x = copy_const_to_operand_aux1_x s,
+        copy_const_to_operand_aux1_diff = copy_const_to_operand_aux1_diff s,
+        copy_const_to_operand_aux1_op = copy_const_to_operand_aux1_op s,
+        copy_const_to_operand_aux1_ret = copy_const_to_operand_aux1_ret'\<rparr>
+in
+ t)"
+
+abbreviation "copy_const_to_operand_aux1_IMP_vars \<equiv>
+  {copy_const_to_operand_aux1_op_str, copy_const_to_operand_aux1_diff_str,
+  copy_const_to_operand_aux1_x_str, copy_const_to_operand_aux1_ret_str}"
+
+definition "copy_const_to_operand_aux1_imp_to_HOL_state p s\<equiv> 
+  \<lparr>copy_const_to_operand_aux1_x = s (add_prefix p copy_const_to_operand_aux1_x_str),
+  copy_const_to_operand_aux1_diff = s (add_prefix p copy_const_to_operand_aux1_diff_str),
+  copy_const_to_operand_aux1_op = s (add_prefix p copy_const_to_operand_aux1_op_str),
+  copy_const_to_operand_aux1_ret = s (add_prefix p copy_const_to_operand_aux1_ret_str)\<rparr>"
+
+lemmas copy_const_to_operand_aux1_state_translators=
+copy_const_to_operand_aux1_imp_to_HOL_state_def
+cons_imp_to_HOL_state_def
+prod_encode_imp_to_HOL_state_def
+operand_bit_to_var_tail_imp_to_HOL_state_def
+nth_bit_tail_imp_to_HOL_state_def
+
+definition "copy_const_to_operand_aux1_IMP_Minus \<equiv> 
+   (nth_bit_tail_prefix @ nth_bit_tail_acc_str) 
+     ::= A (V copy_const_to_operand_aux1_x_str);;
+   (nth_bit_tail_prefix @ nth_bit_tail_n_str) 
+     ::= A (V copy_const_to_operand_aux1_diff_str);;
+   (nth_bit_tail_prefix @ nth_bit_tail_ret_str) 
+     ::= A (N 0);;
+   invoke_subprogram nth_bit_tail_prefix nth_bit_tail_IMP_Minus;;
+
+   (cons_prefix @ cons_h_str) ::= A (V (nth_bit_tail_prefix @ nth_bit_tail_ret_str));;
+   (cons_prefix @ cons_t_str) ::= A (N 0);;
+   (cons_prefix @ cons_ret_str) ::= A (N 0);;
+   invoke_subprogram cons_prefix cons_IMP_Minus;;
+
+   (prod_encode_prefix @ prod_encode_a_str) ::= A (V copy_const_to_operand_aux1_op_str);;
+   (prod_encode_prefix @ prod_encode_b_str) ::= A (V copy_const_to_operand_aux1_diff_str);;
+   (prod_encode_prefix @ prod_encode_ret_str) ::= A (N 0);;
+   invoke_subprogram prod_encode_prefix prod_encode_IMP_Minus;;
+
+   (operand_bit_to_var_tail_prefix @ operand_bit_to_var_tail_n_str)
+     ::= A (V (prod_encode_prefix @ prod_encode_ret_str));;
+   (operand_bit_to_var_tail_prefix @ operand_bit_to_var_tail_ret_str)
+     ::= A (N 0);;
+    invoke_subprogram operand_bit_to_var_tail_prefix operand_bit_to_var_tail_IMP_Minus;;
+
+   (cons_prefix @ cons_h_str) 
+     ::= A (V (operand_bit_to_var_tail_prefix @ operand_bit_to_var_tail_ret_str));;
+   (cons_prefix @ cons_t_str) ::= A (V (cons_prefix @ cons_ret_str));;
+   (cons_prefix @ cons_ret_str) ::= A (N 0);;
+   invoke_subprogram cons_prefix cons_IMP_Minus;;
+
+   (cons_prefix @ cons_h_str) ::= A (N 1);;
+   (cons_prefix @ cons_t_str) ::= A (V (cons_prefix @ cons_ret_str));;
+   (cons_prefix @ cons_ret_str) ::= A (N 0);;
+   invoke_subprogram cons_prefix cons_IMP_Minus;;
+
+   copy_const_to_operand_aux1_ret_str ::= A (V (cons_prefix @ cons_ret_str))
+  "
+
+lemma copy_const_to_operand_aux1_IMP_Minus_correct_function:
+  "(invoke_subprogram p copy_const_to_operand_aux1_IMP_Minus, s) \<Rightarrow>\<^bsup>t\<^esup> s' \<Longrightarrow>
+     s' (add_prefix p copy_const_to_operand_aux1_ret_str)
+      = copy_const_to_operand_aux1_ret
+          (copy_const_to_operand_aux1_imp (copy_const_to_operand_aux1_imp_to_HOL_state p s))"
+  apply (simp only: copy_const_to_operand_aux1_imp_def)
+  apply (simp only: copy_const_to_operand_aux1_IMP_Minus_def prefix_simps)
+  apply (erule Seq_E)+
+  apply (erule nth_bit_tail_IMP_Minus_correct[where vars=copy_const_to_operand_aux1_IMP_vars])
+  subgoal premises p using p(24) by fastforce
+  apply (erule cons_IMP_Minus_correct[where vars=copy_const_to_operand_aux1_IMP_vars])
+  subgoal premises p using p(26) by fastforce
+  apply (erule prod_encode_IMP_Minus_correct[where vars="copy_const_to_operand_aux1_IMP_vars \<union> {cons_prefix @ cons_ret_str}"])
+  subgoal premises p using p(28) by fastforce
+  apply (erule operand_bit_to_var_tail_IMP_Minus_correct[where vars="copy_const_to_operand_aux1_IMP_vars \<union> {cons_prefix @ cons_ret_str}"])
+  subgoal premises p using p(30) by fastforce
+  apply (erule cons_IMP_Minus_correct[where vars=copy_const_to_operand_aux1_IMP_vars])
+  subgoal premises p using p(32) by fastforce
+  apply (erule cons_IMP_Minus_correct[where vars=copy_const_to_operand_aux1_IMP_vars])
+  subgoal premises p using p(34) by fastforce
+  apply (force simp: Let_def copy_const_to_operand_aux1_state_translators)
+  done 
+
+lemma copy_const_to_operand_aux1_IMP_Minus_correct_time:
+  "(invoke_subprogram p copy_const_to_operand_aux1_IMP_Minus, s) \<Rightarrow>\<^bsup>t\<^esup> s' \<Longrightarrow>
+    t =  (copy_const_to_operand_aux1_imp_time 0 (copy_const_to_operand_aux1_imp_to_HOL_state p s))"
+  apply (simp only: copy_const_to_operand_aux1_imp_time_def)
+  apply (simp only: copy_const_to_operand_aux1_IMP_Minus_def prefix_simps)
+  apply (erule Seq_tE)+
+  apply (erule nth_bit_tail_IMP_Minus_correct[where vars=copy_const_to_operand_aux1_IMP_vars])
+  subgoal premises p using p(47) by fastforce
+  apply (erule cons_IMP_Minus_correct[where vars=copy_const_to_operand_aux1_IMP_vars])
+  subgoal premises p using p(49) by fastforce
+  apply (erule prod_encode_IMP_Minus_correct[where vars="copy_const_to_operand_aux1_IMP_vars \<union> {cons_prefix @ cons_ret_str}"])
+  subgoal premises p using p(51) by fastforce
+  apply (erule operand_bit_to_var_tail_IMP_Minus_correct[where vars="copy_const_to_operand_aux1_IMP_vars \<union> {cons_prefix @ cons_ret_str}"])
+  subgoal premises p using p(53) by fastforce
+  apply (erule cons_IMP_Minus_correct[where vars=copy_const_to_operand_aux1_IMP_vars])
+  subgoal premises p using p(55) by fastforce
+  apply (erule cons_IMP_Minus_correct[where vars=copy_const_to_operand_aux1_IMP_vars])
+  subgoal premises p using p(57) by fastforce
+  apply (force simp: Let_def copy_const_to_operand_aux1_state_translators)
+  done 
+
+lemma copy_const_to_operand_aux1_IMP_Minus_correct_effects:
+  "\<lbrakk>(invoke_subprogram (p @ copy_const_to_operand_aux1_pref) copy_const_to_operand_aux1_IMP_Minus, s) \<Rightarrow>\<^bsup>t\<^esup> s';
+    v \<in> vars; \<not> (prefix copy_const_to_operand_aux1_pref v)\<rbrakk>
+   \<Longrightarrow> s (add_prefix p v) = s' (add_prefix p v)"
+  using com_add_prefix_valid'' com_only_vars prefix_def
+  by blast
+
+lemma copy_const_to_operand_aux1_IMP_Minus_correct:
+  "\<lbrakk>(invoke_subprogram (p1 @ p2) copy_const_to_operand_aux1_IMP_Minus, s) \<Rightarrow>\<^bsup>t\<^esup> s';
+    \<And>v. v \<in> vars \<Longrightarrow> \<not> (set p2 \<subseteq> set v);
+    \<lbrakk>t = (copy_const_to_operand_aux1_imp_time 0 (copy_const_to_operand_aux1_imp_to_HOL_state (p1 @ p2) s));
+     s' (add_prefix (p1 @ p2) copy_const_to_operand_aux1_ret_str) =
+          copy_const_to_operand_aux1_ret (copy_const_to_operand_aux1_imp
+                                        (copy_const_to_operand_aux1_imp_to_HOL_state (p1 @ p2) s));
+     \<And>v. v \<in> vars \<Longrightarrow> s (add_prefix p1 v) = s' (add_prefix p1 v)\<rbrakk>
+   \<Longrightarrow> P\<rbrakk> \<Longrightarrow> P"
+  using copy_const_to_operand_aux1_IMP_Minus_correct_function
+  by (auto simp: copy_const_to_operand_aux1_IMP_Minus_correct_time)
+    (meson copy_const_to_operand_aux1_IMP_Minus_correct_effects set_mono_prefix) 
+
+
+subsubsection copy_const_to_operand_acc
+
+record copy_const_to_operand_acc_state = 
+  copy_const_to_operand_acc_acc::nat
+  copy_const_to_operand_acc_diff::nat 
+  copy_const_to_operand_acc_i::nat
+  copy_const_to_operand_acc_op::nat
+  copy_const_to_operand_acc_x::nat
+  copy_const_to_operand_acc_ret::nat
+
+abbreviation "copy_const_to_operand_acc_prefix \<equiv> ''copy_const_to_operand_acc.''"
+abbreviation "copy_const_to_operand_acc_acc_str \<equiv> ''acc''"
+abbreviation "copy_const_to_operand_acc_diff_str \<equiv> ''diff''"
+abbreviation "copy_const_to_operand_acc_i_str \<equiv> ''i''"
+abbreviation "copy_const_to_operand_acc_op_str \<equiv> ''op''"
+abbreviation "copy_const_to_operand_acc_x_str \<equiv> ''x''"
+abbreviation "copy_const_to_operand_acc_ret_str \<equiv> ''ret''"
+
+definition "copy_const_to_operand_acc_state_upd s \<equiv> 
+ (let
+  cons_h' = copy_const_to_operand_acc_acc s;
+  cons_t' = 0;
+  cons_ret' = 0;
+  cons_state = \<lparr>cons_h = cons_h', cons_t = cons_t', cons_ret = cons_ret'\<rparr>;
+  cons_ret_state = cons_imp cons_state;
+
+  copy_const_to_operand_aux1_x' = copy_const_to_operand_acc_x s;
+  copy_const_to_operand_aux1_diff' = copy_const_to_operand_acc_i s - copy_const_to_operand_acc_diff s;
+  copy_const_to_operand_aux1_op'= copy_const_to_operand_acc_op s;
+  copy_const_to_operand_aux1_ret' = 0;
+  copy_const_to_operand_aux1_state = 
+    \<lparr>copy_const_to_operand_aux1_x = copy_const_to_operand_aux1_x',
+    copy_const_to_operand_aux1_diff = copy_const_to_operand_aux1_diff',
+    copy_const_to_operand_aux1_op = copy_const_to_operand_aux1_op',
+    copy_const_to_operand_aux1_ret = copy_const_to_operand_aux1_ret'\<rparr>;
+  copy_const_to_operand_aux1_ret_state = copy_const_to_operand_aux1_imp copy_const_to_operand_aux1_state;
+
+  cons_h' = copy_const_to_operand_aux1_ret copy_const_to_operand_aux1_ret_state;
+  cons_t' = cons_ret cons_ret_state;
+  cons_ret' = 0;
+  cons_state = \<lparr>cons_h = cons_h', cons_t = cons_t', cons_ret = cons_ret'\<rparr>;
+  cons_ret_state = cons_imp cons_state;
+
+  cons_h' = 2;
+  cons_t' = cons_ret cons_ret_state;
+  cons_ret' = 0;
+  cons_state = \<lparr>cons_h = cons_h', cons_t = cons_t', cons_ret = cons_ret'\<rparr>;
+  cons_ret_state = cons_imp cons_state;
+
+  copy_const_to_operand_acc_acc' = cons_ret cons_ret_state;
+  copy_const_to_operand_acc_diff' = copy_const_to_operand_acc_diff s - 1;
+  ret = 
+   \<lparr>copy_const_to_operand_acc_acc = copy_const_to_operand_acc_acc',
+   copy_const_to_operand_acc_diff = copy_const_to_operand_acc_diff',
+   copy_const_to_operand_acc_i = copy_const_to_operand_acc_i s,
+   copy_const_to_operand_acc_op = copy_const_to_operand_acc_op s,
+   copy_const_to_operand_acc_x = copy_const_to_operand_acc_x s,
+   copy_const_to_operand_acc_ret = copy_const_to_operand_acc_ret s\<rparr>
+ in
+  ret)"
+
+definition "copy_const_to_operand_acc_imp_compute_loop_condition s \<equiv> 
+  (let 
+    cond = copy_const_to_operand_acc_diff s
+   in 
+    cond)"
+
+definition "copy_const_to_operand_acc_imp_after_loop s \<equiv> 
+(let
+  copy_const_to_operand_acc_ret' = copy_const_to_operand_acc_acc s;
+  ret = 
+   \<lparr>copy_const_to_operand_acc_acc = copy_const_to_operand_acc_acc s,
+   copy_const_to_operand_acc_diff = copy_const_to_operand_acc_diff s,
+   copy_const_to_operand_acc_i = copy_const_to_operand_acc_i s,
+   copy_const_to_operand_acc_op = copy_const_to_operand_acc_op s,
+   copy_const_to_operand_acc_x = copy_const_to_operand_acc_x s,
+   copy_const_to_operand_acc_ret = copy_const_to_operand_acc_ret'\<rparr>
+in 
+   ret)"
+
+lemmas copy_const_to_operand_acc_imp_subprogram_simps = 
+  copy_const_to_operand_acc_state_upd_def
+  copy_const_to_operand_acc_imp_compute_loop_condition_def
+  copy_const_to_operand_acc_imp_after_loop_def
+
+function copy_const_to_operand_acc_imp::
+  "copy_const_to_operand_acc_state \<Rightarrow> copy_const_to_operand_acc_state" where
+  "copy_const_to_operand_acc_imp s =
+  (if copy_const_to_operand_acc_imp_compute_loop_condition s \<noteq> 0
+   then
+    let next_iteration = copy_const_to_operand_acc_imp (copy_const_to_operand_acc_state_upd s)
+    in next_iteration
+   else
+    let ret = copy_const_to_operand_acc_imp_after_loop s
+    in ret
+  )"
+  by simp+
+termination
+  apply (relation "measure copy_const_to_operand_acc_diff")
+  apply (simp add: copy_const_to_operand_acc_imp_subprogram_simps
+    cons_imp_correct copy_const_to_operand_aux1_imp_correct Let_def)+
+  done
+
+declare copy_const_to_operand_acc_imp.simps [simp del]
+
+lemma copy_const_to_operand_acc_imp_correct:
+  "copy_const_to_operand_acc_ret (copy_const_to_operand_acc_imp s) =
+    copy_const_to_operand_acc (copy_const_to_operand_acc_acc s) (copy_const_to_operand_acc_diff s)
+    (copy_const_to_operand_acc_i s) (copy_const_to_operand_acc_op s) (copy_const_to_operand_acc_x s)"
+  apply (induction s rule: copy_const_to_operand_acc_imp.induct)
+  apply (subst copy_const_to_operand_acc_imp.simps)
+  apply (subst copy_const_to_operand_acc.simps)
+  apply (auto simp del: copy_const_to_operand_acc.simps 
+  simp add: copy_const_to_operand_acc_imp_subprogram_simps Let_def
+  cons_imp_correct copy_const_to_operand_aux1_imp_correct)
+  done  
+
+definition "copy_const_to_operand_acc_state_upd_time t s \<equiv> 
+ (let
+  cons_h' = copy_const_to_operand_acc_acc s;
+  t = t + 2;
+  cons_t' = 0;
+  t = t + 2;
+  cons_ret' = 0;
+  t = t + 2;
+  cons_state = \<lparr>cons_h = cons_h', cons_t = cons_t', cons_ret = cons_ret'\<rparr>;
+  cons_ret_state = cons_imp cons_state;
+  t = t + cons_imp_time 0 cons_state;
+
+  copy_const_to_operand_aux1_x' = copy_const_to_operand_acc_x s;
+  t = t + 2;
+  copy_const_to_operand_aux1_diff' = copy_const_to_operand_acc_i s - copy_const_to_operand_acc_diff s;
+  t = t + 2;
+  copy_const_to_operand_aux1_op'= copy_const_to_operand_acc_op s;
+  t = t + 2;
+  copy_const_to_operand_aux1_ret' = 0;
+  t = t + 2;
+  copy_const_to_operand_aux1_state = 
+    \<lparr>copy_const_to_operand_aux1_x = copy_const_to_operand_aux1_x',
+    copy_const_to_operand_aux1_diff = copy_const_to_operand_aux1_diff',
+    copy_const_to_operand_aux1_op = copy_const_to_operand_aux1_op',
+    copy_const_to_operand_aux1_ret = copy_const_to_operand_aux1_ret'\<rparr>;
+  copy_const_to_operand_aux1_ret_state = copy_const_to_operand_aux1_imp copy_const_to_operand_aux1_state;
+  t = t + copy_const_to_operand_aux1_imp_time 0 copy_const_to_operand_aux1_state;
+
+  cons_h' = copy_const_to_operand_aux1_ret copy_const_to_operand_aux1_ret_state;
+  t = t + 2;
+  cons_t' = cons_ret cons_ret_state;
+  t = t + 2;
+  cons_ret' = 0;
+  t = t + 2;
+  cons_state = \<lparr>cons_h = cons_h', cons_t = cons_t', cons_ret = cons_ret'\<rparr>;
+  cons_ret_state = cons_imp cons_state;
+  t = t + cons_imp_time 0 cons_state;
+
+  cons_h' = 2;
+  t = t + 2;
+  cons_t' = cons_ret cons_ret_state;
+  t = t + 2;
+  cons_ret' = 0;
+  t = t + 2;
+  cons_state = \<lparr>cons_h = cons_h', cons_t = cons_t', cons_ret = cons_ret'\<rparr>;
+  cons_ret_state = cons_imp cons_state;
+  t = t + cons_imp_time 0 cons_state;
+
+  copy_const_to_operand_acc_acc' = cons_ret cons_ret_state;
+  t = t + 2;
+  copy_const_to_operand_acc_diff' = copy_const_to_operand_acc_diff s - 1;
+  t = t + 2;
+  ret = 
+   \<lparr>copy_const_to_operand_acc_acc = copy_const_to_operand_acc_acc',
+   copy_const_to_operand_acc_diff = copy_const_to_operand_acc_diff',
+   copy_const_to_operand_acc_i = copy_const_to_operand_acc_i s,
+   copy_const_to_operand_acc_op = copy_const_to_operand_acc_op s,
+   copy_const_to_operand_acc_x = copy_const_to_operand_acc_x s,
+   copy_const_to_operand_acc_ret = copy_const_to_operand_acc_ret s\<rparr>
+ in
+  t)"
+
+definition "copy_const_to_operand_acc_imp_compute_loop_condition_time t s \<equiv> 
+  (let 
+    cond = copy_const_to_operand_acc_diff s;
+    t = t + 2
+   in 
+    t)"
+
+definition "copy_const_to_operand_acc_imp_after_loop_time t s \<equiv> 
+(let
+  copy_const_to_operand_acc_ret' = copy_const_to_operand_acc_acc s;
+  t = t + 2;
+  ret = 
+   \<lparr>copy_const_to_operand_acc_acc = copy_const_to_operand_acc_acc s,
+   copy_const_to_operand_acc_diff = copy_const_to_operand_acc_diff s,
+   copy_const_to_operand_acc_i = copy_const_to_operand_acc_i s,
+   copy_const_to_operand_acc_op = copy_const_to_operand_acc_op s,
+   copy_const_to_operand_acc_x = copy_const_to_operand_acc_x s,
+   copy_const_to_operand_acc_ret = copy_const_to_operand_acc_ret'\<rparr>
+in 
+   t)"
+
+lemmas copy_const_to_operand_acc_imp_subprogram_time_simps = 
+  copy_const_to_operand_acc_state_upd_time_def
+  copy_const_to_operand_acc_imp_compute_loop_condition_time_def
+  copy_const_to_operand_acc_imp_after_loop_time_def
+  copy_const_to_operand_acc_imp_subprogram_simps
+
+function copy_const_to_operand_acc_imp_time::
+  "nat \<Rightarrow> copy_const_to_operand_acc_state \<Rightarrow> nat" where
+  "copy_const_to_operand_acc_imp_time t s =
+  copy_const_to_operand_acc_imp_compute_loop_condition_time 0 s +
+  (if copy_const_to_operand_acc_imp_compute_loop_condition s \<noteq> 0
+    then
+      (let
+        t = t + 1;
+        next_iteration =
+          copy_const_to_operand_acc_imp_time (t + copy_const_to_operand_acc_state_upd_time 0 s)
+                         (copy_const_to_operand_acc_state_upd s)
+       in next_iteration)
+    else
+      (let
+        t = t + 2;
+        ret = t + copy_const_to_operand_acc_imp_after_loop_time 0 s
+       in ret)
+  )"
+  by auto
+termination
+  apply (relation "measure (copy_const_to_operand_acc_diff \<circ> snd)")
+  by (simp add: copy_const_to_operand_acc_imp_subprogram_time_simps 
+  copy_const_to_operand_aux1_imp_correct cons_imp_correct Let_def)+
+
+
+declare copy_const_to_operand_acc_imp_time.simps [simp del]            
+
+lemma copy_const_to_operand_acc_imp_time_acc:
+  "(copy_const_to_operand_acc_imp_time (Suc t) s) = Suc (copy_const_to_operand_acc_imp_time t s)"
+  by (induction t s rule: copy_const_to_operand_acc_imp_time.induct)
+    ((subst (1 2) copy_const_to_operand_acc_imp_time.simps);
+      (simp add: copy_const_to_operand_acc_state_upd_def))            
+
+lemma copy_const_to_operand_acc_imp_time_acc_2_aux:
+  "(copy_const_to_operand_acc_imp_time t s) = t + (copy_const_to_operand_acc_imp_time 0 s)"
+  by (induction t arbitrary: s) (simp add: copy_const_to_operand_acc_imp_time_acc)+            
+
+lemma copy_const_to_operand_acc_imp_time_acc_2:
+  "t \<noteq> 0 \<Longrightarrow> (copy_const_to_operand_acc_imp_time t s) = t + (copy_const_to_operand_acc_imp_time 0 s)"
+  by (rule copy_const_to_operand_acc_imp_time_acc_2_aux)            
+
+lemma copy_const_to_operand_acc_imp_time_acc_3:
+  "(copy_const_to_operand_acc_imp_time (a + b) s) = a + (copy_const_to_operand_acc_imp_time b s)"
+  by (induction a arbitrary: b s) (simp add: copy_const_to_operand_acc_imp_time_acc)+            
+
+abbreviation "copy_const_to_operand_acc_while_cond \<equiv> ''condition''"
+
+definition "copy_const_to_operand_acc_IMP_init_while_cond \<equiv>
+  copy_const_to_operand_acc_while_cond ::= A (V copy_const_to_operand_acc_diff_str)
+"
+
+definition "copy_const_to_operand_acc_IMP_loop_body \<equiv> 
+(cons_prefix @ cons_h_str) ::= A (V copy_const_to_operand_acc_acc_str);;
+(cons_prefix @ cons_t_str) ::= A (N 0);;
+(cons_prefix @ cons_ret_str) ::= A (N 0);;
+invoke_subprogram cons_prefix cons_IMP_Minus;;
+
+(copy_const_to_operand_aux1_prefix @ copy_const_to_operand_aux1_x_str)
+  ::= A (V copy_const_to_operand_acc_x_str);;
+(copy_const_to_operand_aux1_prefix @ copy_const_to_operand_aux1_diff_str)
+  ::= Sub (V copy_const_to_operand_acc_i_str) (V copy_const_to_operand_acc_diff_str);;
+(copy_const_to_operand_aux1_prefix @ copy_const_to_operand_aux1_op_str)
+  ::= A (V copy_const_to_operand_acc_op_str);;
+  (copy_const_to_operand_aux1_prefix @ copy_const_to_operand_aux1_ret_str)
+  ::= A (N 0);;
+invoke_subprogram copy_const_to_operand_aux1_prefix copy_const_to_operand_aux1_IMP_Minus;;
+ 
+(cons_prefix @ cons_h_str) 
+  ::= A (V (copy_const_to_operand_aux1_prefix @ copy_const_to_operand_aux1_ret_str));;
+(cons_prefix @ cons_t_str) ::= A (V (cons_prefix @ cons_ret_str));;
+(cons_prefix @ cons_ret_str) ::= A (N 0);;
+invoke_subprogram cons_prefix cons_IMP_Minus;;
+
+(cons_prefix @ cons_h_str) ::= A (N 2);;
+(cons_prefix @ cons_t_str) ::= A (V (cons_prefix @ cons_ret_str));;
+(cons_prefix @ cons_ret_str) ::= A (N 0);;
+invoke_subprogram cons_prefix cons_IMP_Minus;;
+
+copy_const_to_operand_acc_acc_str ::= A (V (cons_prefix @ cons_ret_str));;
+copy_const_to_operand_acc_diff_str ::= Sub (V copy_const_to_operand_acc_diff_str) (N 1)"
+
+definition "copy_const_to_operand_acc_IMP_after_loop \<equiv>
+copy_const_to_operand_acc_ret_str ::= A (V copy_const_to_operand_acc_acc_str)
+"
+
+definition copy_const_to_operand_acc_IMP_Minus where
+  "copy_const_to_operand_acc_IMP_Minus \<equiv>
+  copy_const_to_operand_acc_IMP_init_while_cond;;
+  WHILE copy_const_to_operand_acc_while_cond \<noteq>0 DO (
+    copy_const_to_operand_acc_IMP_loop_body;;
+    copy_const_to_operand_acc_IMP_init_while_cond
+  );;
+  copy_const_to_operand_acc_IMP_after_loop"
+
+abbreviation "copy_const_to_operand_acc_IMP_vars\<equiv>
+  {copy_const_to_operand_acc_ret_str, copy_const_to_operand_acc_acc_str,
+  copy_const_to_operand_acc_i_str, copy_const_to_operand_acc_diff_str,
+  copy_const_to_operand_acc_op_str, copy_const_to_operand_acc_x_str,
+  copy_const_to_operand_acc_while_cond}"
+
+lemmas copy_const_to_operand_acc_IMP_subprogram_simps =
+  copy_const_to_operand_acc_IMP_init_while_cond_def
+  copy_const_to_operand_acc_IMP_loop_body_def
+  copy_const_to_operand_acc_IMP_after_loop_def
+
+definition "copy_const_to_operand_acc_imp_to_HOL_state p s =
+  \<lparr>copy_const_to_operand_acc_acc = (s (add_prefix p copy_const_to_operand_acc_acc_str)),
+   copy_const_to_operand_acc_diff = (s (add_prefix p copy_const_to_operand_acc_diff_str)),
+   copy_const_to_operand_acc_i = (s (add_prefix p copy_const_to_operand_acc_i_str)),
+   copy_const_to_operand_acc_op = (s (add_prefix p copy_const_to_operand_acc_op_str)),
+   copy_const_to_operand_acc_x = (s (add_prefix p copy_const_to_operand_acc_x_str)),
+   copy_const_to_operand_acc_ret = (s (add_prefix p copy_const_to_operand_acc_ret_str))\<rparr>"
+
+lemmas copy_const_to_operand_acc_state_translators =
+  copy_const_to_operand_acc_imp_to_HOL_state_def
+  copy_const_to_operand_aux1_imp_to_HOL_state_def
+  cons_imp_to_HOL_state_def
+
+lemmas copy_const_to_operand_acc_complete_simps =
+  copy_const_to_operand_acc_IMP_subprogram_simps
+  copy_const_to_operand_acc_imp_subprogram_simps
+  copy_const_to_operand_acc_state_translators
+
+lemma copy_const_to_operand_acc_IMP_Minus_correct_function:
+  "(invoke_subprogram p copy_const_to_operand_acc_IMP_Minus, s) \<Rightarrow>\<^bsup>t\<^esup> s' \<Longrightarrow>
+     s' (add_prefix p copy_const_to_operand_acc_ret_str)
+      = copy_const_to_operand_acc_ret
+          (copy_const_to_operand_acc_imp (copy_const_to_operand_acc_imp_to_HOL_state p s))"
+  apply(induction "copy_const_to_operand_acc_imp_to_HOL_state p s" arbitrary: s s' t
+    rule: copy_const_to_operand_acc_imp.induct)
+  apply(subst copy_const_to_operand_acc_imp.simps)
+  apply(simp only: copy_const_to_operand_acc_IMP_Minus_def prefix_simps)
+  apply(erule Seq_E)+
+  apply(erule While_tE)
+
+  subgoal
+    apply(simp only: copy_const_to_operand_acc_IMP_subprogram_simps prefix_simps)
+    by(fastforce simp: copy_const_to_operand_acc_IMP_subprogram_simps
+        copy_const_to_operand_acc_imp_subprogram_simps
+        copy_const_to_operand_acc_state_translators)
+
+  apply(erule Seq_E)+
+  apply(dest_com_gen)
+
+  subgoal
+      apply(simp only: copy_const_to_operand_acc_IMP_init_while_cond_def prefix_simps)
+      by(fastforce simp add: copy_const_to_operand_acc_complete_simps)
+
+  subgoal
+      apply(subst (asm) copy_const_to_operand_acc_IMP_init_while_cond_def)
+      apply(simp only: copy_const_to_operand_acc_IMP_loop_body_def prefix_simps)
+      apply(erule Seq_E)+
+      apply(erule cons_IMP_Minus_correct[where vars = "copy_const_to_operand_acc_IMP_vars"])
+      subgoal premises p using p(24) by fastforce
+      apply(erule copy_const_to_operand_aux1_IMP_Minus_correct[where 
+        vars = "copy_const_to_operand_acc_IMP_vars \<union> {cons_prefix @ cons_ret_str}"])
+      subgoal premises p using p(26) by fastforce
+      apply(erule cons_IMP_Minus_correct[where vars = "copy_const_to_operand_acc_IMP_vars"])
+      subgoal premises p using p(28) by fastforce
+      apply(erule cons_IMP_Minus_correct[where vars = "copy_const_to_operand_acc_IMP_vars"])
+      subgoal premises p using p(30) by fastforce
+      by (force simp: copy_const_to_operand_acc_imp_subprogram_simps
+          copy_const_to_operand_acc_state_translators Let_def)
+
+  subgoal
+      apply(simp only: copy_const_to_operand_acc_IMP_init_while_cond_def prefix_simps
+          copy_const_to_operand_acc_IMP_loop_body_def)
+      apply(erule Seq_E)+
+      apply(erule cons_IMP_Minus_correct[where vars = "copy_const_to_operand_acc_IMP_vars"])
+      subgoal premises p using p(24) by fastforce
+      apply(erule copy_const_to_operand_aux1_IMP_Minus_correct[where 
+        vars = "copy_const_to_operand_acc_IMP_vars \<union> {cons_prefix @ cons_ret_str}"])
+      subgoal premises p using p(26) by fastforce
+      apply(erule cons_IMP_Minus_correct[where vars = "copy_const_to_operand_acc_IMP_vars"])
+      subgoal premises p using p(28) by fastforce
+      apply(erule cons_IMP_Minus_correct[where vars = "copy_const_to_operand_acc_IMP_vars"])
+      subgoal premises p using p(30) by fastforce
+      by (force simp: copy_const_to_operand_acc_imp_subprogram_simps
+          copy_const_to_operand_acc_state_translators Let_def)
+  done        
+
+lemma copy_const_to_operand_acc_IMP_Minus_correct_effects:
+  "\<lbrakk>(invoke_subprogram (p @ copy_const_to_operand_acc_pref) copy_const_to_operand_acc_IMP_Minus, s) \<Rightarrow>\<^bsup>t\<^esup> s';
+    v \<in> vars; \<not> (prefix copy_const_to_operand_acc_pref v)\<rbrakk>
+   \<Longrightarrow> s (add_prefix p v) = s' (add_prefix p v)"
+  using com_add_prefix_valid'' com_only_vars prefix_def
+  by blast            
+
+lemmas copy_const_to_operand_acc_complete_time_simps =
+  copy_const_to_operand_acc_imp_subprogram_time_simps
+  copy_const_to_operand_acc_imp_time_acc_2
+  copy_const_to_operand_acc_imp_time_acc_3
+  copy_const_to_operand_acc_state_translators
+
+lemma copy_const_to_operand_acc_IMP_Minus_correct_time:
+  "(invoke_subprogram p copy_const_to_operand_acc_IMP_Minus, s) \<Rightarrow>\<^bsup>t\<^esup> s' \<Longrightarrow>
+     t = copy_const_to_operand_acc_imp_time 0 (copy_const_to_operand_acc_imp_to_HOL_state p s)"
+  apply(induction "copy_const_to_operand_acc_imp_to_HOL_state p s" arbitrary: s s' t
+      rule: copy_const_to_operand_acc_imp.induct)
+  apply(subst copy_const_to_operand_acc_imp_time.simps)
+  apply(simp only: copy_const_to_operand_acc_IMP_Minus_def prefix_simps)
+
+  apply(erule Seq_tE)+
+  apply(erule While_tE_time)
+
+  subgoal
+    apply(simp only: copy_const_to_operand_acc_IMP_subprogram_simps prefix_simps)
+    by (force simp: copy_const_to_operand_acc_IMP_subprogram_simps
+        copy_const_to_operand_acc_imp_subprogram_time_simps copy_const_to_operand_acc_state_translators)
+
+  apply(erule Seq_tE)+
+  apply(simp add: add.assoc)
+  apply(dest_com_gen_time)
+
+  subgoal
+    apply(simp only: copy_const_to_operand_acc_IMP_init_while_cond_def prefix_simps)
+    by(fastforce simp add: copy_const_to_operand_acc_complete_simps)
+
+  subgoal
+    apply(subst (asm) copy_const_to_operand_acc_IMP_init_while_cond_def)
+    apply(simp only: copy_const_to_operand_acc_IMP_loop_body_def prefix_simps)
+    apply(erule Seq_E)+
+    apply(erule cons_IMP_Minus_correct[where vars = "copy_const_to_operand_acc_IMP_vars"])
+    subgoal premises p using p(27) by fastforce
+    apply(erule copy_const_to_operand_aux1_IMP_Minus_correct[where 
+      vars = "copy_const_to_operand_acc_IMP_vars \<union> {cons_prefix @ cons_ret_str}"])
+    subgoal premises p using p(29) by fastforce
+    apply(erule cons_IMP_Minus_correct[where vars = "copy_const_to_operand_acc_IMP_vars"])
+    subgoal premises p using p(31) by fastforce
+    apply(erule cons_IMP_Minus_correct[where vars = "copy_const_to_operand_acc_IMP_vars"])
+    subgoal premises p using p(33) by fastforce
+    by (force simp: copy_const_to_operand_acc_imp_subprogram_simps
+        copy_const_to_operand_acc_state_translators Let_def)
+  
+  subgoal
+    apply(simp only: prefix_simps copy_const_to_operand_acc_IMP_init_while_cond_def
+        copy_const_to_operand_acc_IMP_loop_body_def)
+    apply(erule Seq_tE)+
+    apply(erule cons_IMP_Minus_correct[where vars = "copy_const_to_operand_acc_IMP_vars"])
+    subgoal premises p using p(45) by fastforce
+    apply(erule copy_const_to_operand_aux1_IMP_Minus_correct[where 
+      vars = "copy_const_to_operand_acc_IMP_vars \<union> {cons_prefix @ cons_ret_str}"])
+    subgoal premises p using p(47) by fastforce
+    apply(erule cons_IMP_Minus_correct[where vars = "copy_const_to_operand_acc_IMP_vars"])
+    subgoal premises p using p(49) by fastforce
+    apply(erule cons_IMP_Minus_correct[where vars = "copy_const_to_operand_acc_IMP_vars"])
+    subgoal premises p using p(51) by fastforce
+    by(force simp: copy_const_to_operand_acc_complete_time_simps Let_def)
+ done      
+
+lemma copy_const_to_operand_acc_IMP_Minus_correct:
+  "\<lbrakk>(invoke_subprogram (p1 @ p2) copy_const_to_operand_acc_IMP_Minus, s) \<Rightarrow>\<^bsup>t\<^esup> s';
+    \<And>v. v \<in> vars \<Longrightarrow> \<not> (set p2 \<subseteq> set v);
+    \<lbrakk>t = (copy_const_to_operand_acc_imp_time 0 (copy_const_to_operand_acc_imp_to_HOL_state (p1 @ p2) s));
+     s' (add_prefix (p1 @ p2) copy_const_to_operand_acc_ret_str) =
+          copy_const_to_operand_acc_ret (copy_const_to_operand_acc_imp
+                                        (copy_const_to_operand_acc_imp_to_HOL_state (p1 @ p2) s));
+     \<And>v. v \<in> vars \<Longrightarrow> s (add_prefix p1 v) = s' (add_prefix p1 v)\<rbrakk>
+   \<Longrightarrow> P\<rbrakk> \<Longrightarrow> P"
+  using copy_const_to_operand_acc_IMP_Minus_correct_function
+  by (auto simp: copy_const_to_operand_acc_IMP_Minus_correct_time)
+    (meson copy_const_to_operand_acc_IMP_Minus_correct_effects set_mono_prefix)
+
+subsubsection copy_const_to_operand_tail
+
+record copy_const_to_operand_tail_state = 
+  copy_const_to_operand_tail_i::nat
+  copy_const_to_operand_tail_op::nat
+  copy_const_to_operand_tail_x::nat
+  copy_const_to_operand_tail_ret::nat
+
+abbreviation "copy_const_to_operand_tail_prefix \<equiv> ''copy_const_to_operand_tail.''"
+abbreviation "copy_const_to_operand_tail_i_str \<equiv> ''i''"
+abbreviation "copy_const_to_operand_tail_op_str \<equiv> ''op''"
+abbreviation "copy_const_to_operand_tail_x_str \<equiv> ''x''"
+abbreviation "copy_const_to_operand_tail_ret_str \<equiv> ''ret''"
+
+function copy_const_to_operand_tail_imp 
+  :: "copy_const_to_operand_tail_state \<Rightarrow> copy_const_to_operand_tail_state" where 
+"copy_const_to_operand_tail_imp s = 
+  (let
+    cons_h' = 0;
+    cons_t' = 0;
+    cons_ret' = 0;
+    cons_state = \<lparr>cons_h = cons_h', cons_t = cons_t', cons_ret = cons_ret'\<rparr>;
+    cons_ret_state = cons_imp cons_state;
+
+    copy_const_to_operand_acc_acc' = cons_ret cons_ret_state;
+    copy_const_to_operand_acc_diff' = copy_const_to_operand_tail_i s;
+    copy_const_to_operand_acc_i' = copy_const_to_operand_tail_i s;
+    copy_const_to_operand_acc_op' = copy_const_to_operand_tail_op s;
+    copy_const_to_operand_acc_x' = copy_const_to_operand_tail_x s;
+    copy_const_to_operand_acc_ret' = 0;
+    copy_const_to_operand_acc_state = 
+      \<lparr>copy_const_to_operand_acc_acc = copy_const_to_operand_acc_acc',
+      copy_const_to_operand_acc_diff = copy_const_to_operand_acc_diff',
+      copy_const_to_operand_acc_i = copy_const_to_operand_acc_i',
+      copy_const_to_operand_acc_op = copy_const_to_operand_acc_op',
+      copy_const_to_operand_acc_x = copy_const_to_operand_acc_x',
+      copy_const_to_operand_acc_ret = copy_const_to_operand_acc_ret'\<rparr>;
+    copy_const_to_operand_acc_ret_state
+      = copy_const_to_operand_acc_imp copy_const_to_operand_acc_state;
+    copy_const_to_operand_tail_ret' = 
+      copy_const_to_operand_acc_ret copy_const_to_operand_acc_ret_state;
+    ret =
+      \<lparr>copy_const_to_operand_tail_i = copy_const_to_operand_tail_i s,
+      copy_const_to_operand_tail_op = copy_const_to_operand_tail_op s,
+      copy_const_to_operand_tail_x = copy_const_to_operand_tail_x s,
+      copy_const_to_operand_tail_ret = copy_const_to_operand_tail_ret'\<rparr>
+  in 
+   ret)" by simp+
+  termination 
+  by (relation "measure copy_const_to_operand_tail_i", simp)
+
+declare copy_const_to_operand_tail_imp.simps[simp del]
+
+lemma copy_const_to_operand_tail_imp_correct:
+  "copy_const_to_operand_tail_ret (copy_const_to_operand_tail_imp s)
+    = copy_const_to_operand_tail (copy_const_to_operand_tail_i s) 
+      (copy_const_to_operand_tail_op s) (copy_const_to_operand_tail_x s)"
+apply (simp only: copy_const_to_operand_tail_imp.simps)
+apply (auto simp add: copy_const_to_operand_acc_imp_correct cons_imp_correct Let_def
+  copy_const_to_operand_tail_def)
+done 
+
+function copy_const_to_operand_tail_imp_time 
+  :: "nat \<Rightarrow> copy_const_to_operand_tail_state \<Rightarrow> nat" where 
+"copy_const_to_operand_tail_imp_time t s = 
+  (let
+    cons_h' = 0;
+    t = t + 2;
+    cons_t' = 0;
+    t = t + 2;
+    cons_ret' = 0;
+    t = t + 2;
+    cons_state = \<lparr>cons_h = cons_h', cons_t = cons_t', cons_ret = cons_ret'\<rparr>;
+    cons_ret_state = cons_imp cons_state;
+    t = t + cons_imp_time 0 cons_state;
+
+    copy_const_to_operand_acc_acc' = cons_ret cons_ret_state;
+    t = t + 2;
+    copy_const_to_operand_acc_diff' = copy_const_to_operand_tail_i s;
+    t = t + 2;
+    copy_const_to_operand_acc_i' = copy_const_to_operand_tail_i s;
+    t = t + 2;
+    copy_const_to_operand_acc_op' = copy_const_to_operand_tail_op s;
+    t = t + 2;
+    copy_const_to_operand_acc_x' = copy_const_to_operand_tail_x s;
+    t = t + 2;
+    copy_const_to_operand_acc_ret' = 0;
+    t = t + 2;
+    copy_const_to_operand_acc_state = 
+      \<lparr>copy_const_to_operand_acc_acc = copy_const_to_operand_acc_acc',
+      copy_const_to_operand_acc_diff = copy_const_to_operand_acc_diff',
+      copy_const_to_operand_acc_i = copy_const_to_operand_acc_i',
+      copy_const_to_operand_acc_op = copy_const_to_operand_acc_op',
+      copy_const_to_operand_acc_x = copy_const_to_operand_acc_x',
+      copy_const_to_operand_acc_ret = copy_const_to_operand_acc_ret'\<rparr>;
+    copy_const_to_operand_acc_ret_state
+      = copy_const_to_operand_acc_imp copy_const_to_operand_acc_state;
+    t = t + copy_const_to_operand_acc_imp_time 0 copy_const_to_operand_acc_state;
+
+    copy_const_to_operand_tail_ret' = 
+      copy_const_to_operand_acc_ret copy_const_to_operand_acc_ret_state;
+    t = t + 2;
+    ret =
+      \<lparr>copy_const_to_operand_tail_i = copy_const_to_operand_tail_i s,
+      copy_const_to_operand_tail_op = copy_const_to_operand_tail_op s,
+      copy_const_to_operand_tail_x = copy_const_to_operand_tail_x s,
+      copy_const_to_operand_tail_ret = copy_const_to_operand_tail_ret'\<rparr>
+  in 
+   t)" by auto
+  termination 
+  by (relation "measure (copy_const_to_operand_tail_i \<circ> snd)", simp)
+
+abbreviation "copy_const_to_operand_tail_IMP_vars \<equiv> 
+  {copy_const_to_operand_tail_i_str, copy_const_to_operand_tail_op_str,
+  copy_const_to_operand_tail_x_str, copy_const_to_operand_tail_ret_str}"
+
+definition "copy_const_to_operand_tail_imp_to_HOL_state p s \<equiv> 
+   \<lparr>copy_const_to_operand_tail_i = s (add_prefix p copy_const_to_operand_tail_i_str),
+    copy_const_to_operand_tail_op = s (add_prefix p copy_const_to_operand_tail_op_str),
+    copy_const_to_operand_tail_x = s (add_prefix p copy_const_to_operand_tail_x_str),
+    copy_const_to_operand_tail_ret = s (add_prefix p copy_const_to_operand_tail_ret_str)\<rparr>"
+
+lemmas copy_const_to_operand_tail_state_translators=
+  copy_const_to_operand_tail_imp_to_HOL_state_def
+  copy_const_to_operand_acc_imp_to_HOL_state_def
+  cons_imp_to_HOL_state_def
+
+definition "copy_const_to_operand_tail_IMP_Minus \<equiv> 
+  (cons_prefix @ cons_h_str) ::= A (N 0);;
+  (cons_prefix @ cons_t_str) ::= A (N 0);;
+  (cons_prefix @ cons_ret_str) ::= A (N 0);;
+  invoke_subprogram cons_prefix cons_IMP_Minus;;
+  
+  (copy_const_to_operand_acc_prefix @ copy_const_to_operand_acc_acc_str)
+    ::= A (V (cons_prefix @ cons_ret_str));;
+  (copy_const_to_operand_acc_prefix @ copy_const_to_operand_acc_diff_str)
+    ::= A (V copy_const_to_operand_tail_i_str);;
+  (copy_const_to_operand_acc_prefix @ copy_const_to_operand_acc_i_str)
+    ::= A (V copy_const_to_operand_tail_i_str);;
+  (copy_const_to_operand_acc_prefix @ copy_const_to_operand_acc_op_str)
+    ::= A (V copy_const_to_operand_tail_op_str);;
+  (copy_const_to_operand_acc_prefix @ copy_const_to_operand_acc_x_str)
+    ::= A (V copy_const_to_operand_tail_x_str);;
+  (copy_const_to_operand_acc_prefix @ copy_const_to_operand_acc_ret_str)
+    ::= A (N 0);;
+  invoke_subprogram copy_const_to_operand_acc_prefix copy_const_to_operand_acc_IMP_Minus;;
+  copy_const_to_operand_tail_ret_str 
+    ::= A (V (copy_const_to_operand_acc_prefix @ copy_const_to_operand_acc_ret_str))"
+
+lemma copy_const_to_operand_tail_IMP_Minus_correct_function:
+  "(invoke_subprogram p copy_const_to_operand_tail_IMP_Minus, s) \<Rightarrow>\<^bsup>t\<^esup> s' \<Longrightarrow>
+     s' (add_prefix p copy_const_to_operand_tail_ret_str)
+      = copy_const_to_operand_tail_ret
+          (copy_const_to_operand_tail_imp (copy_const_to_operand_tail_imp_to_HOL_state p s))"
+  apply (simp only: copy_const_to_operand_tail_imp.simps)
+  apply (simp only: copy_const_to_operand_tail_IMP_Minus_def prefix_simps)
+  apply (erule Seq_E)+
+  apply (erule cons_IMP_Minus_correct[where vars = copy_const_to_operand_tail_IMP_vars])
+  subgoal premises p using p(12) by fastforce
+  apply (erule copy_const_to_operand_acc_IMP_Minus_correct[where vars = copy_const_to_operand_tail_IMP_vars])
+  subgoal premises p using p(14) by fastforce
+  apply (force simp: copy_const_to_operand_tail_state_translators Let_def)
+  done 
+
+lemma copy_const_to_operand_tail_IMP_Minus_correct_effects:
+  "\<lbrakk>(invoke_subprogram (p @ copy_const_to_operand_acc_pref) copy_const_to_operand_acc_IMP_Minus, s) \<Rightarrow>\<^bsup>t\<^esup> s';
+    v \<in> vars; \<not> (prefix copy_const_to_operand_acc_pref v)\<rbrakk>
+   \<Longrightarrow> s (add_prefix p v) = s' (add_prefix p v)"
+  using com_add_prefix_valid'' com_only_vars prefix_def
+  by blast            
+
+lemma copy_const_to_operand_tail_IMP_Minus_correct_time:
+  "(invoke_subprogram p copy_const_to_operand_tail_IMP_Minus, s) \<Rightarrow>\<^bsup>t\<^esup> s' \<Longrightarrow>
+     t = copy_const_to_operand_tail_imp_time 0 (copy_const_to_operand_tail_imp_to_HOL_state p s)"
+  apply (simp only: copy_const_to_operand_tail_imp_time.simps)
+  apply (simp only: copy_const_to_operand_tail_IMP_Minus_def prefix_simps)
+  apply (erule Seq_tE)+
+  apply (erule cons_IMP_Minus_correct[where vars = copy_const_to_operand_tail_IMP_vars])
+  subgoal premises p using p(23) by fastforce
+  apply (erule copy_const_to_operand_acc_IMP_Minus_correct[where vars = copy_const_to_operand_tail_IMP_vars])
+  subgoal premises p using p(25) by fastforce
+  apply (force simp: copy_const_to_operand_tail_state_translators Let_def)
+  done 
+
+lemma copy_const_to_operand_tail_IMP_Minus_correct:
+  "\<lbrakk>(invoke_subprogram (p1 @ p2) copy_const_to_operand_tail_IMP_Minus, s) \<Rightarrow>\<^bsup>t\<^esup> s';
+    \<And>v. v \<in> vars \<Longrightarrow> \<not> (set p2 \<subseteq> set v);
+    \<lbrakk>t = (copy_const_to_operand_tail_imp_time 0 (copy_const_to_operand_tail_imp_to_HOL_state (p1 @ p2) s));
+     s' (add_prefix (p1 @ p2) copy_const_to_operand_tail_ret_str) =
+          copy_const_to_operand_tail_ret (copy_const_to_operand_tail_imp
+                                        (copy_const_to_operand_tail_imp_to_HOL_state (p1 @ p2) s));
+     \<And>v. v \<in> vars \<Longrightarrow> s (add_prefix p1 v) = s' (add_prefix p1 v)\<rbrakk>
+   \<Longrightarrow> P\<rbrakk> \<Longrightarrow> P"
+  using copy_const_to_operand_tail_IMP_Minus_correct_function 
+      copy_const_to_operand_tail_IMP_Minus_correct_time
+       set_mono_prefix
+  by (smt (verit, ccfv_SIG) com_add_prefix_valid_subset com_only_vars)
+
+subsection copy_atom_to_operand_nat
+
+record copy_atom_to_operand_nat_state = 
+  copy_atom_to_operand_nat_n::nat
+  copy_atom_to_operand_nat_op::nat
+  copy_atom_to_operand_nat_a::nat
+  copy_atom_to_operand_nat_ret::nat
+
+abbreviation "copy_atom_to_operand_nat_prefix \<equiv> ''copy_atom_to_operand_nat.''"
+abbreviation "copy_atom_to_operand_nat_n_str \<equiv> ''n''"
+abbreviation "copy_atom_to_operand_nat_op_str \<equiv> ''op''"
+abbreviation "copy_atom_to_operand_nat_a_str \<equiv> ''a''"
+abbreviation "copy_atom_to_operand_nat_ret_str \<equiv> ''ret''"
+abbreviation "copy_atom_to_operand_nat_cond \<equiv> ''cond''"
+
+function copy_atom_to_operand_nat_imp 
+  :: "copy_atom_to_operand_nat_state \<Rightarrow> copy_atom_to_operand_nat_state"
+where 
+"copy_atom_to_operand_nat_imp s = 
+(let
+  fst'_state_p' = copy_atom_to_operand_nat_a s;
+  fst'_state = \<lparr>fst'_state_p = fst'_state_p'\<rparr>;
+  fst'_ret_state = fst'_imp fst'_state;
+  cond = fst'_state_p fst'_ret_state
+in
+  (if cond \<noteq> 0 
+  then (let
+         snd'_state_p' = copy_atom_to_operand_nat_a s;
+         snd'_state = \<lparr>snd'_state_p = snd'_state_p'\<rparr>;
+         snd'_ret_state = snd'_imp snd'_state;
+         
+         copy_const_to_operand_tail_i' = copy_atom_to_operand_nat_n s;
+         copy_const_to_operand_tail_op' = copy_atom_to_operand_nat_op s;
+         copy_const_to_operand_tail_x' = snd'_state_p snd'_ret_state;
+         copy_const_to_operand_tail_ret' = 0;
+         copy_const_to_operand_tail_state 
+           = \<lparr>copy_const_to_operand_tail_i = copy_const_to_operand_tail_i',
+             copy_const_to_operand_tail_op = copy_const_to_operand_tail_op',
+             copy_const_to_operand_tail_x = copy_const_to_operand_tail_x',
+             copy_const_to_operand_tail_ret = copy_const_to_operand_tail_ret'\<rparr>;
+         copy_const_to_operand_tail_ret_state = 
+            copy_const_to_operand_tail_imp copy_const_to_operand_tail_state;
+         copy_atom_to_operand_nat_ret' 
+            = copy_const_to_operand_tail_ret copy_const_to_operand_tail_ret_state;
+         ret =
+           \<lparr>copy_atom_to_operand_nat_n = copy_atom_to_operand_nat_n s,
+            copy_atom_to_operand_nat_op = copy_atom_to_operand_nat_op s,
+            copy_atom_to_operand_nat_a = copy_atom_to_operand_nat_a s,
+            copy_atom_to_operand_nat_ret = copy_atom_to_operand_nat_ret'\<rparr>
+        in
+         ret)
+  else (let
+         snd'_state_p' = copy_atom_to_operand_nat_a s;
+         snd'_state = \<lparr>snd'_state_p = snd'_state_p'\<rparr>;
+         snd'_ret_state = snd'_imp snd'_state;
+         
+         copy_var_to_operand_tail_i' = copy_atom_to_operand_nat_n s;
+         copy_var_to_operand_tail_op' = copy_atom_to_operand_nat_op s;
+         copy_var_to_operand_tail_v' = snd'_state_p snd'_ret_state;
+         copy_var_to_operand_tail_ret' = 0;
+         copy_var_to_operand_tail_state 
+           = \<lparr>copy_var_to_operand_tail_i = copy_var_to_operand_tail_i',
+             copy_var_to_operand_tail_op = copy_var_to_operand_tail_op',
+             copy_var_to_operand_tail_v = copy_var_to_operand_tail_v',
+             copy_var_to_operand_tail_ret = copy_var_to_operand_tail_ret'\<rparr>;
+         copy_var_to_operand_tail_ret_state = 
+            copy_var_to_operand_tail_imp copy_var_to_operand_tail_state;
+         copy_atom_to_operand_nat_ret' 
+            = copy_var_to_operand_tail_ret copy_var_to_operand_tail_ret_state;
+         ret =
+           \<lparr>copy_atom_to_operand_nat_n = copy_atom_to_operand_nat_n s,
+            copy_atom_to_operand_nat_op = copy_atom_to_operand_nat_op s,
+            copy_atom_to_operand_nat_a = copy_atom_to_operand_nat_a s,
+            copy_atom_to_operand_nat_ret = copy_atom_to_operand_nat_ret'\<rparr>
+        in
+         ret)
+  ))" by simp+
+termination by (relation "measure copy_atom_to_operand_nat_n", simp)
+
+declare copy_atom_to_operand_nat_imp.simps[simp del]
+
+lemma copy_atom_to_operand_nat_imp_correct[let_function_correctness]:
+  "copy_atom_to_operand_nat_ret (copy_atom_to_operand_nat_imp s) = 
+    copy_atom_to_operand_nat (copy_atom_to_operand_nat_n s)
+      (copy_atom_to_operand_nat_op s) (copy_atom_to_operand_nat_a s)"
+apply (simp only: copy_atom_to_operand_nat_imp.simps)
+apply (simp add: copy_var_to_operand_tail_imp_correct
+copy_const_to_operand_tail_imp_correct fst'_imp_correct snd'_imp_correct Let_def)
+by (simp add: fst_nat_fst'_nat snd_nat_snd'_nat copy_atom_to_operand_nat_def
+subtail_copy_const_to_operand subtail_copy_var_to_operand)
+
+function copy_atom_to_operand_nat_imp_time 
+  :: "nat \<Rightarrow> copy_atom_to_operand_nat_state \<Rightarrow> nat"
+where 
+"copy_atom_to_operand_nat_imp_time t s = 
+(let
+  fst'_state_p' = copy_atom_to_operand_nat_a s;
+  t = t + 2;
+  fst'_state = \<lparr>fst'_state_p = fst'_state_p'\<rparr>;
+  fst'_ret_state = fst'_imp fst'_state;
+  t = t + fst'_imp_time 0 fst'_state;
+  cond = fst'_state_p fst'_ret_state;
+  t = t + 2
+in
+  (if cond \<noteq> 0 
+  then (let
+         t = t + 1;
+         snd'_state_p' = copy_atom_to_operand_nat_a s;
+         t = t + 2;
+         snd'_state = \<lparr>snd'_state_p = snd'_state_p'\<rparr>;
+         snd'_ret_state = snd'_imp snd'_state;
+         t = t + snd'_imp_time 0 snd'_state;
+         
+         copy_const_to_operand_tail_i' = copy_atom_to_operand_nat_n s;
+         t = t + 2;
+         copy_const_to_operand_tail_op' = copy_atom_to_operand_nat_op s;
+         t = t + 2;
+         copy_const_to_operand_tail_x' = snd'_state_p snd'_ret_state;
+         t = t + 2;
+         copy_const_to_operand_tail_ret' = 0;
+         t = t + 2;
+         copy_const_to_operand_tail_state 
+           = \<lparr>copy_const_to_operand_tail_i = copy_const_to_operand_tail_i',
+             copy_const_to_operand_tail_op = copy_const_to_operand_tail_op',
+             copy_const_to_operand_tail_x = copy_const_to_operand_tail_x',
+             copy_const_to_operand_tail_ret = copy_const_to_operand_tail_ret'\<rparr>;
+         copy_const_to_operand_tail_ret_state = 
+            copy_const_to_operand_tail_imp copy_const_to_operand_tail_state;
+         t = t + copy_const_to_operand_tail_imp_time 0 copy_const_to_operand_tail_state;
+         copy_atom_to_operand_nat_ret' 
+            = copy_const_to_operand_tail_ret copy_const_to_operand_tail_ret_state;
+         t = t + 2;
+         ret =
+           \<lparr>copy_atom_to_operand_nat_n = copy_atom_to_operand_nat_n s,
+            copy_atom_to_operand_nat_op = copy_atom_to_operand_nat_op s,
+            copy_atom_to_operand_nat_a = copy_atom_to_operand_nat_a s,
+            copy_atom_to_operand_nat_ret = copy_atom_to_operand_nat_ret'\<rparr>
+        in
+         t)
+  else (let
+         t = t + 1;
+         snd'_state_p' = copy_atom_to_operand_nat_a s;
+         t = t + 2;
+         snd'_state = \<lparr>snd'_state_p = snd'_state_p'\<rparr>;
+         snd'_ret_state = snd'_imp snd'_state;
+         t = t + snd'_imp_time 0 snd'_state;
+         
+         copy_var_to_operand_tail_i' = copy_atom_to_operand_nat_n s;
+         t = t + 2;
+         copy_var_to_operand_tail_op' = copy_atom_to_operand_nat_op s;
+         t = t + 2;
+         copy_var_to_operand_tail_v' = snd'_state_p snd'_ret_state;
+         t = t + 2;
+         copy_var_to_operand_tail_ret' = 0;
+         t = t + 2;
+         copy_var_to_operand_tail_state 
+           = \<lparr>copy_var_to_operand_tail_i = copy_var_to_operand_tail_i',
+             copy_var_to_operand_tail_op = copy_var_to_operand_tail_op',
+             copy_var_to_operand_tail_v = copy_var_to_operand_tail_v',
+             copy_var_to_operand_tail_ret = copy_var_to_operand_tail_ret'\<rparr>;
+         copy_var_to_operand_tail_ret_state = 
+            copy_var_to_operand_tail_imp copy_var_to_operand_tail_state;
+         t = t + copy_var_to_operand_tail_imp_time 0 copy_var_to_operand_tail_state;
+         copy_atom_to_operand_nat_ret' 
+            = copy_var_to_operand_tail_ret copy_var_to_operand_tail_ret_state;
+         t = t + 2;
+         ret =
+           \<lparr>copy_atom_to_operand_nat_n = copy_atom_to_operand_nat_n s,
+            copy_atom_to_operand_nat_op = copy_atom_to_operand_nat_op s,
+            copy_atom_to_operand_nat_a = copy_atom_to_operand_nat_a s,
+            copy_atom_to_operand_nat_ret = copy_atom_to_operand_nat_ret'\<rparr>
+        in
+         t)
+  ))" by auto
+termination by (relation "measure (copy_atom_to_operand_nat_n \<circ> snd)", simp)
+
+declare copy_atom_to_operand_nat_imp_time.simps[simp del]
+
+abbreviation "copy_atom_to_operand_nat_IMP_vars \<equiv> 
+ {copy_atom_to_operand_nat_ret_str, copy_atom_to_operand_nat_n_str,
+ copy_atom_to_operand_nat_op_str, copy_atom_to_operand_nat_a_str,
+ copy_atom_to_operand_nat_cond}"
+
+definition "copy_atom_to_operand_nat_imp_to_HOL_state p s\<equiv> 
+\<lparr>copy_atom_to_operand_nat_n = s (add_prefix p copy_atom_to_operand_nat_n_str),
+copy_atom_to_operand_nat_op = s (add_prefix p copy_atom_to_operand_nat_op_str),
+copy_atom_to_operand_nat_a = s (add_prefix p copy_atom_to_operand_nat_a_str),
+copy_atom_to_operand_nat_ret = s (add_prefix p copy_atom_to_operand_nat_ret_str)\<rparr>"
+
+lemmas copy_atom_to_operand_nat_state_translators=
+  copy_atom_to_operand_nat_imp_to_HOL_state_def
+  copy_var_to_operand_tail_imp_to_HOL_state_def
+  copy_const_to_operand_tail_imp_to_HOL_state_def
+  fst'_imp_to_HOL_state_def snd'_imp_to_HOL_state_def
+
+definition "copy_atom_to_operand_nat_IMP_Minus \<equiv> 
+  (fst'_prefix @ fst'_p_str) ::= A (V copy_atom_to_operand_nat_a_str);;
+  invoke_subprogram fst'_prefix fst'_IMP_Minus;;
+  copy_atom_to_operand_nat_cond ::= A (V (fst'_prefix @ fst'_p_str));;
+  IF copy_atom_to_operand_nat_cond\<noteq>0 
+  THEN 
+    (
+    (snd'_prefix @ snd'_p_str) ::= A (V copy_atom_to_operand_nat_a_str);;
+    invoke_subprogram snd'_prefix snd'_IMP_Minus;;
+
+    (copy_const_to_operand_tail_prefix @ copy_const_to_operand_tail_i_str)
+      ::= A (V copy_atom_to_operand_nat_n_str);;
+    (copy_const_to_operand_tail_prefix @ copy_const_to_operand_tail_op_str)
+      ::= A (V copy_atom_to_operand_nat_op_str);;
+    (copy_const_to_operand_tail_prefix @ copy_const_to_operand_tail_x_str)
+      ::= A (V (snd'_prefix @ snd'_p_str));;
+    (copy_const_to_operand_tail_prefix @ copy_const_to_operand_tail_ret_str)
+      ::= A (N 0);;
+    invoke_subprogram copy_const_to_operand_tail_prefix copy_const_to_operand_tail_IMP_Minus;;
+
+    (copy_atom_to_operand_nat_ret_str) ::=
+      A (V (copy_const_to_operand_tail_prefix @ copy_const_to_operand_tail_ret_str))
+    )
+  ELSE 
+    (
+    (snd'_prefix @ snd'_p_str) ::= A (V copy_atom_to_operand_nat_a_str);;
+    invoke_subprogram snd'_prefix snd'_IMP_Minus;;
+
+    (copy_var_to_operand_tail_prefix @ copy_var_to_operand_tail_i_str)
+      ::= A (V copy_atom_to_operand_nat_n_str);;
+    (copy_var_to_operand_tail_prefix @ copy_var_to_operand_tail_op_str)
+      ::= A (V copy_atom_to_operand_nat_op_str);;
+    (copy_var_to_operand_tail_prefix @ copy_var_to_operand_tail_v_str)
+      ::= A (V (snd'_prefix @ snd'_p_str));;
+    (copy_var_to_operand_tail_prefix @ copy_var_to_operand_tail_ret_str)
+      ::= A (N 0);;
+    invoke_subprogram copy_var_to_operand_tail_prefix copy_var_to_operand_tail_IMP_Minus;;
+
+    (copy_atom_to_operand_nat_ret_str) ::=
+      A (V (copy_var_to_operand_tail_prefix @ copy_var_to_operand_tail_ret_str))
+    )
+  "
+
+lemma copy_atom_to_operand_nat_IMP_Minus_correct_function:
+  "(invoke_subprogram p copy_atom_to_operand_nat_IMP_Minus, s) \<Rightarrow>\<^bsup>t\<^esup> s' \<Longrightarrow>
+     s' (add_prefix p copy_atom_to_operand_nat_ret_str)
+      = copy_atom_to_operand_nat_ret
+          (copy_atom_to_operand_nat_imp (copy_atom_to_operand_nat_imp_to_HOL_state p s))"
+  apply (simp only: copy_atom_to_operand_nat_imp.simps)
+  apply (simp only: copy_atom_to_operand_nat_IMP_Minus_def prefix_simps)
+  apply (erule Seq_E)+
+  apply (erule fst'_IMP_Minus_correct[where vars = copy_atom_to_operand_nat_IMP_vars])
+  subgoal premises p using p(4) by fastforce
+  apply (erule If_E)
+    subgoal 
+      apply (erule Seq_E)+
+      apply (erule snd'_IMP_Minus_correct[where vars = copy_atom_to_operand_nat_IMP_vars])
+      subgoal premises p using p (14) by fastforce
+      apply (erule copy_const_to_operand_tail_IMP_Minus_correct[where vars = copy_atom_to_operand_nat_IMP_vars])
+      subgoal premises p using p (16) by fastforce
+      apply (force simp: copy_atom_to_operand_nat_state_translators Let_def)
+    done 
+
+    subgoal 
+      apply (erule Seq_E)+
+      apply (erule snd'_IMP_Minus_correct[where vars = copy_atom_to_operand_nat_IMP_vars])
+      subgoal premises p using p (14) by fastforce
+      apply (erule copy_var_to_operand_tail_IMP_Minus_correct[where vars = copy_atom_to_operand_nat_IMP_vars])
+      subgoal premises p using p (16) by fastforce
+      apply (force simp: copy_atom_to_operand_nat_state_translators Let_def)
+    done 
+  done 
+
+lemma copy_atom_to_operand_nat_IMP_Minus_correct_time:
+  "(invoke_subprogram p copy_atom_to_operand_nat_IMP_Minus, s) \<Rightarrow>\<^bsup>t\<^esup> s' \<Longrightarrow>
+    t = (copy_atom_to_operand_nat_imp_time 0 (copy_atom_to_operand_nat_imp_to_HOL_state p s))"
+  apply (simp only: copy_atom_to_operand_nat_imp_time.simps)
+  apply (simp only: copy_atom_to_operand_nat_IMP_Minus_def prefix_simps)
+  apply (erule Seq_tE)+
+  apply (erule fst'_IMP_Minus_correct[where vars = copy_atom_to_operand_nat_IMP_vars])
+  subgoal premises p using p(7) by fastforce
+  apply (erule If_tE)
+    subgoal 
+      apply (erule Seq_tE)+
+      apply (erule snd'_IMP_Minus_correct[where vars = copy_atom_to_operand_nat_IMP_vars])
+      subgoal premises p using p (25) by fastforce
+      apply (erule copy_const_to_operand_tail_IMP_Minus_correct[where vars = copy_atom_to_operand_nat_IMP_vars])
+      subgoal premises p using p (27) by fastforce
+      apply (force simp: copy_atom_to_operand_nat_state_translators Let_def)
+    done 
+
+    subgoal 
+      apply (erule Seq_tE)+
+      apply (erule snd'_IMP_Minus_correct[where vars = copy_atom_to_operand_nat_IMP_vars])
+      subgoal premises p using p (25) by fastforce
+      apply (erule copy_var_to_operand_tail_IMP_Minus_correct[where vars = copy_atom_to_operand_nat_IMP_vars])
+      subgoal premises p using p (27) by fastforce
+      apply (force simp: copy_atom_to_operand_nat_state_translators Let_def)
+    done 
+  done 
+
+lemma copy_atom_to_operand_nat_IMP_Minus_correct:
+  "\<lbrakk>(invoke_subprogram (p1 @ p2) copy_atom_to_operand_nat_IMP_Minus, s) \<Rightarrow>\<^bsup>t\<^esup> s';
+    \<And>v. v \<in> vars \<Longrightarrow> \<not> (set p2 \<subseteq> set v);
+    \<lbrakk>t = (copy_atom_to_operand_nat_imp_time 0 (copy_atom_to_operand_nat_imp_to_HOL_state (p1 @ p2) s));
+     s' (add_prefix (p1 @ p2) copy_atom_to_operand_nat_ret_str) =
+          copy_atom_to_operand_nat_ret (copy_atom_to_operand_nat_imp
+                                        (copy_atom_to_operand_nat_imp_to_HOL_state (p1 @ p2) s));
+     \<And>v. v \<in> vars \<Longrightarrow> s (add_prefix p1 v) = s' (add_prefix p1 v)\<rbrakk>
+   \<Longrightarrow> P\<rbrakk> \<Longrightarrow> P"
+  using copy_atom_to_operand_nat_IMP_Minus_correct_function 
+      copy_atom_to_operand_nat_IMP_Minus_correct_time
+       set_mono_prefix
+  by (smt (verit, ccfv_SIG) com_add_prefix_valid_subset com_only_vars)
+
+end 
